Cache.thy
@@ -1,0 +1,1261 @@
+theory Cache
+  imports EventSystem
+begin
+
+
+subsection \<open>Events\<close>
+
+datatype event =
+  ReqS nat | ReqE nat | Inv nat | InvAck nat | SendS nat | SendE nat
+
+datatype state =
+  Invalid | Shared | Exclusive
+
+subsection \<open>Implementation of server\<close>
+
+record server =
+  invset :: "bool list"
+  shrset :: "bool list"
+  curptr :: "nat option"
+  grantE :: bool
+
+record client =
+  st :: state
+
+text \<open>
+  Handler for send shared - change status to shared.
+\<close>
+definition SendS_impl :: "(client, event, unit) event_monad" where
+  "SendS_impl = (
+    get \<bind> (\<lambda>s.
+    put (s\<lparr>st := Shared\<rparr>)))"
+
+theorem SendS_rule:
+  "\<lbrace> \<lambda>s es. s = s0 \<and> es = [] \<rbrace>
+    SendS_impl
+   \<lbrace> \<lambda>_ s es. s = s0\<lparr>st := Shared\<rparr> \<and> es = [] \<rbrace>!"
+  unfolding SendS_impl_def apply wp by auto
+
+text \<open>
+  Handler for send exclusive - change status to exclusive.
+\<close>
+definition SendE_impl :: "(client, event, unit) event_monad" where
+  "SendE_impl = (
+    get \<bind> (\<lambda>s.
+    put (s\<lparr>st := Exclusive\<rparr>)))"
+
+theorem SendE_rule:
+  "\<lbrace> \<lambda>s es. s = s0 \<and> es = [] \<rbrace>
+    SendE_impl
+   \<lbrace> \<lambda>_ s es. s = s0\<lparr>st := Exclusive\<rparr> \<and> es = [] \<rbrace>!"
+  unfolding SendE_impl_def apply wp by auto
+
+text \<open>
+  Handler for invalidate - change status to invalid, then send acknowledgement.
+\<close>
+definition Inv_impl :: "nat \<Rightarrow> (client, event, unit) event_monad" where
+  "Inv_impl i = (
+    get \<bind> (\<lambda>s.
+    put (s\<lparr>st := Invalid\<rparr>) \<bind> (\<lambda>_.
+    signal (InvAck i))))"
+
+theorem Inv_rule:
+  "\<lbrace> \<lambda>s es. s = s0 \<and> es = [] \<rbrace>
+    Inv_impl i
+   \<lbrace> \<lambda>_ s es. s = s0\<lparr>st := Invalid\<rparr> \<and> es = [InvAck i] \<rbrace>!"
+  unfolding Inv_impl_def apply wp by auto
+
+text \<open>
+  Implementation of grant:
+  if invset array becomes all empty, send the appropriate grant.
+\<close>
+definition grant_impl :: "nat \<Rightarrow> (server, event, unit) event_monad" where
+  "grant_impl N = (
+    get \<bind> (\<lambda>s.
+    if curptr s = None then skip else
+      if (\<forall>i. i < N \<longrightarrow> \<not>invset s ! i) then
+        if grantE s then
+          signal (SendE (the (curptr s))) \<bind> (\<lambda>_.
+          put (s\<lparr>curptr := None, shrset := (shrset s)[the (curptr s) := True]\<rparr>))
+        else
+          signal (SendS (the (curptr s))) \<bind> (\<lambda>_.
+          put (s\<lparr>curptr := None, shrset := (shrset s)[the (curptr s) := True]\<rparr>))
+      else skip))"
+
+definition grant :: "nat \<Rightarrow> server \<Rightarrow> server" where
+  "grant N s =
+    (case curptr s of None \<Rightarrow> s | Some j \<Rightarrow>
+      if (\<forall>i. i < N \<longrightarrow> \<not>invset s ! i) then
+        s\<lparr>curptr := None, shrset := (shrset s)[j := True]\<rparr>
+      else s)"
+
+definition grant_ev :: "nat \<Rightarrow> server \<Rightarrow> event list" where
+  "grant_ev N s =
+    (case curptr s of None \<Rightarrow> [] | Some j \<Rightarrow>
+      if (\<forall>i. i < N \<longrightarrow> \<not>invset s ! i) then
+        if grantE s then [SendE j] else [SendS j]
+      else [])"
+
+theorem grant_rule:
+  "\<lbrace> \<lambda>s es. s = s0 \<and> es = [] \<rbrace>
+    grant_impl N
+   \<lbrace> \<lambda>_ s es. s = grant N s0 \<and> es = grant_ev N s0 \<rbrace>!"
+  unfolding grant_impl_def grant_def grant_ev_def
+  apply wp by auto
+
+text \<open>
+  Handler for invack - update the invset array. Then possibly send
+  the appropriate grant.
+\<close>
+definition Invack_impl :: "nat \<Rightarrow> nat \<Rightarrow> (server, event, unit) event_monad" where
+  "Invack_impl N i = (
+    get \<bind> (\<lambda>s.
+    put (s\<lparr>invset := (invset s)[i := False]\<rparr>) \<bind> (\<lambda>_.
+    grant_impl N)))"
+
+theorem Invack_rule:
+  "\<lbrace> \<lambda>s es. s = s0 \<and> es = [] \<rbrace>
+    Invack_impl N i
+   \<lbrace> \<lambda>_ s es. s = grant N (s0\<lparr>invset := (invset s0)[i := False]\<rparr>) \<and>
+              es = grant_ev N (s0\<lparr>invset := (invset s0)[i := False]\<rparr>) \<rbrace>!"
+  unfolding Invack_impl_def
+  apply (rule validNF_bind)
+   prefer 2 apply (rule validNF_bind)
+    prefer 2 apply (rule grant_rule)
+   apply wp apply (rule validNF_weaken_pre)
+  apply wp by auto      
+
+definition sendInv_impl :: "nat \<Rightarrow> (server, event, nat) event_monad" where
+  "sendInv_impl N = (
+    whileLoop (\<lambda>i _. i < N)
+      (\<lambda>i. get \<bind> (\<lambda>s.
+             if shrset s ! i then
+               signal (Inv i) \<bind> (\<lambda>_.
+               put (s\<lparr>shrset := (shrset s)[i := False], invset := (invset s)[i := True]\<rparr>) \<bind> (\<lambda>_.
+               return (Suc i)))
+             else
+               return (Suc i))) 0)"
+
+fun sendInv :: "nat \<Rightarrow> nat \<Rightarrow> server \<Rightarrow> server" where
+  "sendInv N 0 s = s"
+| "sendInv N (Suc i) s =
+   (let s' = sendInv N i s in
+     if shrset s' ! i then
+       s'\<lparr>shrset := (shrset s')[i := False], invset := (invset s')[i := True]\<rparr>
+     else s')"
+
+fun sendInv_ev :: "nat \<Rightarrow> nat \<Rightarrow> server \<Rightarrow> event list" where
+  "sendInv_ev N 0 s = []"
+| "sendInv_ev N (Suc i) s =
+   (let s' = sendInv N i s;
+        es' = sendInv_ev N i s
+    in
+      if shrset s' ! i then
+        es' @ [Inv i]
+      else es')"
+
+theorem sendInv_rule:
+  "\<lbrace> \<lambda>s es. s = s0 \<and> es = [] \<rbrace>
+    sendInv_impl N
+   \<lbrace> \<lambda>i s es. i = N \<and> s = sendInv N N s0 \<and> es = sendInv_ev N N s0 \<rbrace>!"
+  unfolding sendInv_impl_def
+  apply (rule validNF_whileLoop[where
+            I="\<lambda>i s es. i \<le> N \<and> s = sendInv N i s0 \<and> es = sendInv_ev N i s0" and
+            R="measure (\<lambda>(r,s). N - r)"])
+  subgoal for s es by auto
+  subgoal for i s'
+    apply wp by (auto simp add: Let_def)
+  subgoal by auto
+  subgoal for i s es by auto
+  done
+
+definition set_curptr :: "nat \<Rightarrow> bool \<Rightarrow> server \<Rightarrow> server" where
+  "set_curptr i gE s = (s\<lparr>grantE := gE, curptr := Some i\<rparr>)"
+
+lemma set_curptr_rule:
+  "\<lbrace> \<lambda>s es. s = s0 \<and> es = [] \<rbrace>
+     modify (set_curptr i gE)
+   \<lbrace> \<lambda>_ s es. s = set_curptr i gE s0 \<and> es = [] \<rbrace>!"
+  apply wp unfolding set_curptr_def by auto
+
+text \<open>
+  Handler for request shared. If some node has exclusive access, send
+  invalidate messages.
+\<close>
+definition ReqS_impl :: "nat \<Rightarrow> nat \<Rightarrow> (server, event, unit) event_monad" where
+  "ReqS_impl N i = (
+    get \<bind> (\<lambda>s.
+    if grantE s then
+      sendInv_impl N \<bind> (\<lambda>_.
+      modify (set_curptr i False) \<bind> (\<lambda>_.
+      grant_impl N))
+    else
+      signal (SendS i) \<bind> (\<lambda>_.
+      put(s\<lparr>shrset := (shrset s)[i := True]\<rparr>))))"
+
+theorem ReqS_rule:
+  "\<lbrace> \<lambda>s es. s = s0 \<and> es = [] \<rbrace>
+    ReqS_impl N i
+   \<lbrace> \<lambda>_ s es. s = (if grantE s0 then
+                     grant N (set_curptr i False (sendInv N N s0))
+                   else
+                     s0\<lparr>shrset := (shrset s0)[i := True]\<rparr>) \<and>
+              es = (if grantE s0 then sendInv_ev N N s0 @ grant_ev N (set_curptr i False (sendInv N N s0))
+                    else [SendS i]) \<rbrace>!"
+  unfolding ReqS_impl_def apply (rule validNF_bind)
+   apply (rule validNF_get_post)
+  subgoal for r
+    apply (cases "grantE r") apply auto
+    subgoal
+      apply (rule validNF_bind) apply (subst validNF_conj_pre)
+       apply (rule impI) apply (rule sendInv_rule)
+      apply (rule validNF_bind)
+       apply (subst validNF_conj_pre) apply (rule impI)
+       apply (rule validNF_frame2)
+       apply (rule set_curptr_rule)
+      apply (rule validNF_strengthen_post)
+       apply (rule validNF_frame2)
+       apply (rule grant_rule)
+      by auto
+    subgoal unfolding validNF_def valid_def no_fail_def by auto
+    subgoal unfolding validNF_def valid_def no_fail_def by auto
+    subgoal apply wp by auto
+    done
+  done
+
+text \<open>
+  Handler for request exclusive. Always send invalidate messages.
+\<close>
+definition ReqE_impl :: "nat \<Rightarrow> nat \<Rightarrow> (server, event, unit) event_monad" where
+  "ReqE_impl N i = (
+    sendInv_impl N \<bind> (\<lambda>_.
+    modify (set_curptr i True) \<bind> (\<lambda>_.
+    grant_impl N)))"
+
+theorem ReqE_rule:
+  "\<lbrace> \<lambda>s es. s = s0 \<and> es = [] \<rbrace>
+    ReqE_impl N i
+   \<lbrace> \<lambda>_ s es. s = grant N (set_curptr i True (sendInv N N s0)) \<and>
+              es = sendInv_ev N N s0 @ grant_ev N (set_curptr i True (sendInv N N s0)) \<rbrace>!"
+  unfolding ReqE_impl_def
+  apply (rule validNF_bind)
+   apply (rule sendInv_rule)
+  subgoal for N'
+    apply (subst validNF_conj_pre) apply (rule impI)
+    apply (rule validNF_bind)
+     apply (rule validNF_frame2)
+     apply (rule set_curptr_rule)
+    apply (rule validNF_strengthen_post)
+     apply (rule validNF_frame2)
+     apply (rule grant_rule)
+    by auto
+  done
+
+subsection \<open>Verify the event system\<close>
+
+fun system :: "nat \<Rightarrow> (event, server \<times> client list) event_system" where
+  "system N (ReqS i) = Some (apply_fst (ReqS_impl N i))"
+| "system N (ReqE i) = Some (apply_fst (ReqE_impl N i))"
+| "system N (Inv i) = Some (apply_snd (apply_idx (Inv_impl i) i))"
+| "system N (InvAck i) = Some (apply_fst (Invack_impl N i))"
+| "system N (SendS i) = Some (apply_snd (apply_idx SendS_impl i))"
+| "system N (SendE i) = Some (apply_snd (apply_idx SendE_impl i))"
+
+theorem sValidNF_SendS:
+  "sValidNF (system N)
+    (\<lambda>p es. p = (s0, clist) \<and> nil\<^sub>e es)
+    (SendS i)
+    (\<lambda>p es. p = (s0, clist[i := (clist ! i)\<lparr>st := Shared\<rparr>]) \<and> nil\<^sub>e es)"
+  apply (rule sValidNF_Some)
+    apply (rule system.simps)
+  apply (rule validNF_weaken_pre)
+  apply (rule validNF_apply_snd[where R="\<lambda>s. s = s0"])
+    apply (rule validNF_apply_idx[OF SendS_rule])
+   apply (auto simp add: nil_event_def)
+  by (rule sValidNF_list_null)
+
+theorem sValidNF_SendE:
+  "sValidNF (system N)
+    (\<lambda>p es. p = (s0, clist) \<and> nil\<^sub>e es)
+    (SendE i)
+    (\<lambda>p es. p = (s0, clist[i := (clist ! i)\<lparr>st := Exclusive\<rparr>]) \<and> nil\<^sub>e es)"
+  apply (rule sValidNF_Some)
+    apply (rule system.simps)
+  apply (rule validNF_weaken_pre)
+  apply (rule validNF_apply_snd[where R="\<lambda>s. s = s0"])
+    apply (rule validNF_apply_idx[OF SendE_rule])
+   apply (auto simp add: nil_event_def)
+  by (rule sValidNF_list_null)
+
+fun apply_grant :: "nat \<Rightarrow> server \<Rightarrow> server \<times> client list \<Rightarrow> server \<times> client list" where
+  "apply_grant N s1 (s, clist) =
+    (case curptr s1 of None \<Rightarrow> (s, clist) | Some j \<Rightarrow>
+      if (\<forall>i. i < N \<longrightarrow> \<not>invset s1 ! i) then
+        if grantE s1 then (s, clist[j := (clist ! j)\<lparr>st := Exclusive\<rparr>])
+        else (s, clist[j := (clist ! j)\<lparr>st := Shared\<rparr>])
+      else (s, clist))"
+
+lemma sValidNF_list_apply_grant:
+  "sValidNF_list (system N)
+    (\<lambda>p es. p = (s0, clist) \<and> nil\<^sub>e es)
+    (grant_ev N s1)
+    (\<lambda>p es. p = apply_grant N s1 (s0, clist) \<and> nil\<^sub>e es)"
+  apply (cases "curptr s1")
+  subgoal
+    apply (auto simp add: grant_ev_def)
+    by (rule sValidNF_list_null)
+  subgoal for j
+    apply (auto simp add: grant_ev_def)
+    subgoal
+      apply (rule sValidNF_list_single)
+      by (rule sValidNF_SendE)
+    subgoal
+      apply (rule sValidNF_list_single)
+      by (rule sValidNF_SendS)
+    subgoal
+      by (rule sValidNF_list_null)
+    subgoal
+      by (rule sValidNF_list_null)
+    done
+  done
+
+declare apply_grant.simps [simp del]
+
+fun sInvAck :: "nat \<Rightarrow> nat \<Rightarrow> server \<times> client list \<Rightarrow> server \<times> client list" where
+  "sInvAck N i (s0, clist) =
+   (let s1 = s0\<lparr>invset := (invset s0)[i := False]\<rparr> in
+     apply_grant N s1 (grant N s1, clist))"
+
+theorem sValidNF_InvAck:
+  "sValidNF (system N)
+    (\<lambda>p es. p = (s0, clist) \<and> nil\<^sub>e es)
+    (InvAck i)
+    (\<lambda>p es. p = sInvAck N i (s0, clist) \<and> nil\<^sub>e es)"
+  apply (rule sValidNF_Some)
+  apply (rule system.simps)
+   apply (rule validNF_weaken_pre)
+    apply (rule validNF_apply_fst[where R="\<lambda>s. s = clist"])
+    apply (rule Invack_rule)
+   apply (auto simp add: nil_event_def)[1]
+  apply (auto simp add: Let_def)
+  by (rule sValidNF_list_apply_grant)
+
+declare sInvAck.simps [simp del]
+
+fun sInv :: "nat \<Rightarrow> nat \<Rightarrow> server \<times> client list \<Rightarrow> server \<times> client list" where
+  "sInv N i (s0, clist) =
+    sInvAck N i (s0, clist[i := (clist ! i)\<lparr>st := Invalid\<rparr>])"
+
+theorem sValidNF_Inv:
+  "sValidNF (system N)
+    (\<lambda>p es. p = (s0, clist) \<and> nil\<^sub>e es)
+    (Inv i)
+    (\<lambda>p es. p = sInv N i (s0, clist) \<and> nil\<^sub>e es)"
+  apply (rule sValidNF_Some)
+    apply (rule system.simps)
+  apply (rule validNF_weaken_pre)
+  apply (rule validNF_apply_snd[where R="\<lambda>s. s = s0"])
+  apply (rule validNF_apply_idx[OF Inv_rule])
+   apply (auto simp add: nil_event_def)
+  apply (rule sValidNF_list_single)
+  by (rule sValidNF_InvAck[unfolded nil_event_def])
+
+declare sInv.simps [simp del]
+
+\<comment> \<open>Here s1 is the initial server state for generating the sendInv events.
+    (s, clist) is the server/client state the events are applied to\<close>
+fun apply_sendInv :: "nat \<Rightarrow> nat \<Rightarrow> server \<Rightarrow> server \<times> client list \<Rightarrow> server \<times> client list" where
+  "apply_sendInv N 0 s1 (s, clist) = (s, clist)"
+| "apply_sendInv N (Suc i) s1 (s, clist) =
+   (let s1' = sendInv N i s1;
+        (s', clist') = apply_sendInv N i s1 (s, clist)
+    in
+      if shrset s1' ! i then
+        sInv N i (s', clist')
+      else
+        (s', clist'))"
+
+lemma sValidNF_list_sendInv:
+  "sValidNF_list (system N)
+    (\<lambda>p es. p = (s0, clist) \<and> nil\<^sub>e es)
+    (sendInv_ev N i s1)
+    (\<lambda>p es. p = apply_sendInv N i s1 (s0, clist) \<and> nil\<^sub>e es)"
+proof (induction i)
+  case 0
+  then show ?case
+    by (auto intro: sValidNF_list_null)
+next
+  case (Suc i)
+  show ?case
+    apply simp apply (intro conjI impI)
+    subgoal apply (rule sValidNF_list_append)
+      apply (rule Suc)
+      apply (rule sValidNF_list_single)
+      apply (cases "apply_sendInv N i s1 (s0, clist)")
+      apply auto
+      by (rule sValidNF_Inv)
+    subgoal
+      by (rule Suc)
+    done
+qed
+
+declare apply_sendInv.simps [simp del]
+
+fun sReq :: "nat \<Rightarrow> nat \<Rightarrow> bool \<Rightarrow> server \<times> client list \<Rightarrow> server \<times> client list" where
+  "sReq N i b (s0, clist) =
+    (let s1 = set_curptr i b (sendInv N N s0);
+         s2 = grant N s1
+     in
+       apply_grant N s1 (apply_sendInv N N s0 (s2, clist)))"
+
+fun sReqE :: "nat \<Rightarrow> nat \<Rightarrow> server \<times> client list \<Rightarrow> server \<times> client list" where
+  "sReqE N i (s0, clist) = sReq N i True (s0, clist)"
+
+theorem sValidNF_ReqE:
+  "sValidNF (system N)
+    (\<lambda>p es. p = (s0, clist) \<and> nil\<^sub>e es)
+    (ReqE i)
+    (\<lambda>p es. p = sReqE N i (s0, clist) \<and> nil\<^sub>e es)"
+  apply (rule sValidNF_Some)
+    apply (rule system.simps)
+  apply (rule validNF_weaken_pre)
+    apply (rule validNF_apply_fst[where R="\<lambda>s. s = clist"])
+    apply (rule ReqE_rule)
+   apply (auto simp add: nil_event_def)[1]
+  subgoal for p es
+    apply (cases p) apply auto
+    apply (rule sValidNF_list_append)
+     apply (rule sValidNF_list_sendInv)
+    apply (simp only: Let_def)
+    apply (cases "apply_sendInv N N s0 (grant N (set_curptr i True (sendInv N N s0)), clist)")
+    apply auto
+    by (rule sValidNF_list_apply_grant)
+  done
+
+declare sReqE.simps [simp del]
+
+fun sReqS :: "nat \<Rightarrow> nat \<Rightarrow> server \<times> client list \<Rightarrow> server \<times> client list" where
+  "sReqS N i (s0, clist) =
+    (if grantE s0 then
+       sReq N i False (s0, clist)
+     else
+       (s0\<lparr>shrset := (shrset s0)[i := True]\<rparr>, clist[i := (clist ! i)\<lparr>st := Shared\<rparr>]))"
+
+theorem sValidNF_ReqS:
+  "sValidNF (system N)
+    (\<lambda>p es. p = (s0, clist) \<and> nil\<^sub>e es)
+    (ReqS i)
+    (\<lambda>p es. p = sReqS N i (s0, clist) \<and> nil\<^sub>e es)"
+  apply (rule sValidNF_Some)
+    apply (rule system.simps)
+   apply (rule validNF_weaken_pre)
+    apply (rule validNF_apply_fst[where R="\<lambda>s. s = clist"])
+    apply (rule ReqS_rule)
+   apply (auto simp add: nil_event_def)[1]
+  subgoal for p es
+    apply (cases p) apply auto
+    subgoal
+      apply (rule sValidNF_list_append)
+       apply (rule sValidNF_list_sendInv)
+      apply (simp only: Let_def)
+      apply (cases "apply_sendInv N N s0 (grant N (set_curptr i False (sendInv N N s0)), clist)")
+      apply auto
+      by (rule sValidNF_list_apply_grant)
+    subgoal
+      apply (rule sValidNF_list_single)
+      by (rule sValidNF_SendS)
+    done
+  done
+
+subsection \<open>Functional correctness\<close>
+
+fun system_inv1 :: "nat \<Rightarrow> server \<times> client list \<Rightarrow> bool" where
+  "system_inv1 N (s, clist) =
+    (length (shrset s) = N \<and> length (invset s) = N \<and> length clist = N \<and>
+     (case curptr s of None \<Rightarrow> True | Some j \<Rightarrow> j < N) \<and>
+     (\<forall>i<N. (st (clist ! i) = Shared \<or> st (clist ! i) = Exclusive) \<longrightarrow>
+            (shrset s ! i \<or> invset s ! i)))"
+
+lemma sendInv_inv':
+  "i \<le> N \<Longrightarrow> system_inv1 N (s, clist) \<Longrightarrow>
+   system_inv1 N (sendInv N i s, clist)"
+proof (induction i)
+  case 0
+  then show ?case by auto
+next
+  case (Suc i)
+  have a: "i < N" using Suc(2) by auto
+  have b: "length (shrset (sendInv N i s)) = N" using Suc by auto
+  have c: "length (invset (sendInv N i s)) = N" using Suc by auto
+  show ?case
+    unfolding sendInv.simps Let_def
+    apply (cases "shrset (sendInv N i s) ! i")
+    subgoal using b c apply auto
+      subgoal using Suc by auto
+      subgoal using Suc by auto
+      subgoal for i' apply (cases "i' = i")
+        using Suc by (auto simp add: b c)
+      subgoal for i' apply (cases "i' = i")
+        using Suc by (auto simp add: b c)
+      done
+    using Suc by auto
+qed
+
+lemma sendInv_inv:
+  "system_inv1 N (s, clist) \<Longrightarrow> system_inv1 N (sendInv N N s, clist)"
+  using sendInv_inv' by auto
+
+lemma set_curptr_inv:
+  "i < N \<Longrightarrow> system_inv1 N (s, clist) \<Longrightarrow> system_inv1 N (set_curptr i b s, clist)"
+  by (auto simp add: set_curptr_def)
+
+lemma grant_inv:
+  "system_inv1 N (s, clist) \<Longrightarrow>
+   system_inv1 N (grant N s, clist)"
+  apply (cases "curptr s")
+  subgoal by (auto simp add: grant_def)
+  subgoal for j
+    apply (auto simp add: grant_def)
+    subgoal for i apply (cases "i = j") by auto
+    subgoal for i apply (cases "i = j") by auto
+    done
+  done
+
+lemma grant_inv2:
+  "curptr s = Some j \<Longrightarrow> j < N \<Longrightarrow> length (shrset s) = N \<Longrightarrow>
+   \<forall>i. i < N \<longrightarrow> \<not>invset s ! i \<Longrightarrow>
+   shrset (grant N s) ! j"
+  by (auto simp add: grant_def)
+
+lemma apply_grant_inv:
+  "curptr s1 = Some j \<Longrightarrow>
+   (\<forall>i. i < N \<longrightarrow> \<not>invset s1 ! i) \<longrightarrow> shrset s ! j \<Longrightarrow>
+   system_inv1 N (s, clist) \<Longrightarrow>
+   system_inv1 N (apply_grant N s1 (s, clist))"
+  apply (auto simp add: apply_grant.simps)
+  subgoal for i apply (cases "i = j") by auto
+  subgoal for i apply (cases "i = j") by auto
+  subgoal for i apply (cases "i = j") by auto
+  subgoal for i apply (cases "i = j") by auto
+  done
+
+lemma sInv_inv1:
+  assumes "curptr s = Some j"
+    and "system_inv1 N (s, clist)"
+  shows "system_inv1 N (sInv N i (s, clist))"
+proof -
+  let ?s'="s\<lparr>invset := (invset s)[i := False]\<rparr>"
+  have *: "j < N"
+    using assms by auto
+  have a: "curptr ?s' = Some j"
+    using assms(1) by auto
+  have b: "system_inv1 N (apply_grant N ?s' (grant N ?s', clist[i := (clist ! i)\<lparr>st := Invalid\<rparr>]))"
+  proof (cases "\<forall>i. i < N \<longrightarrow> \<not>invset ?s' ! i")
+    case True
+    have b1: "grant N ?s' = ?s'\<lparr>curptr := None, shrset := (shrset ?s')[j := True]\<rparr>"
+      unfolding grant_def a using True by auto
+    show ?thesis 
+      apply (rule apply_grant_inv[where j=j])
+      subgoal using assms(1) by auto
+      subgoal unfolding b1 using * assms(2) by auto
+      subgoal apply (rule grant_inv)
+        using assms(2) apply auto
+        subgoal for j apply (cases "i = j") by auto
+        subgoal for j apply (cases "i = j") by auto
+        done
+      done
+  next
+    case False
+    have b2: "grant N ?s' = ?s'"
+      unfolding grant_def a using False by auto
+    have b3: "apply_grant N ?s' (?s', clist[i := (clist ! i)\<lparr>st := Invalid\<rparr>]) =
+              (?s', clist[i := (clist ! i)\<lparr>st := Invalid\<rparr>])"
+      unfolding apply_grant.simps a using False by auto
+    show ?thesis
+      unfolding b2 b3
+      using assms(2) apply auto
+      subgoal for j apply (cases "i = j") by auto
+      subgoal for j apply (cases "i = j") by auto
+      done
+  qed
+  then show ?thesis
+    by (auto simp add: sInv.simps sInvAck.simps Let_def)
+qed
+
+lemma sInv_inv2:
+  assumes "curptr s = None"
+    and "system_inv1 N (s, clist)"
+  shows "system_inv1 N (sInv N i (s, clist))"
+proof -
+  let ?s'="s\<lparr>invset := (invset s)[i := False]\<rparr>"
+  have a: "curptr ?s' = None"
+    using assms(1) by auto
+  have b: "grant N ?s' = ?s'"
+    by (auto simp add: grant_def assms(1) a)
+  have c: "apply_grant N ?s' (?s', clist[i := (clist ! i)\<lparr>st := Invalid\<rparr>]) =
+           (?s', clist[i := (clist ! i)\<lparr>st := Invalid\<rparr>])"
+    by (auto simp add: apply_grant.simps assms(1))
+  show ?thesis
+    apply (auto simp add: sInv.simps sInvAck.simps Let_def)
+    unfolding b c 
+    using assms(2) apply auto
+    subgoal for j apply (cases "i = j") by auto
+    subgoal for j apply (cases "i = j") by auto
+    done
+qed
+
+lemma sInv_inv:
+  "system_inv1 N (s, clist) \<Longrightarrow> system_inv1 N (sInv N i (s, clist))"
+  apply (cases "curptr s")
+  using sInv_inv1 sInv_inv2 by auto
+
+lemma apply_sendInv_inv:
+  "system_inv1 N (s, clist) \<Longrightarrow>
+   system_inv1 N (apply_sendInv N i s1 (s, clist))"
+proof (induction i)
+  case 0
+  then show ?case
+    by (auto simp add: apply_sendInv.simps)
+next
+  case (Suc i)
+  show ?case
+    unfolding apply_sendInv.simps Let_def
+    apply (cases "shrset (sendInv N i s1) ! i")
+    subgoal apply auto
+      apply (cases "apply_sendInv N i s1 (s, clist)")
+      by (metis Suc.IH Suc.prems sInv_inv)
+    using Suc by auto
+qed
+
+lemma sendInv_shrset_same:
+  assumes "system_inv1 N (s0, clist)"
+  shows "j \<ge> i \<Longrightarrow> shrset (sendInv N i s0) ! j = shrset s0 ! j \<and> invset (sendInv N i s0) ! j = invset s0 ! j"
+  apply (induction i) by (auto simp add: Let_def)
+
+\<comment> \<open>The following lemmas prove results about shrset and invset\<close>
+lemma sendInv_shrset:
+  assumes "system_inv1 N (s0, clist)"
+    and "\<forall>i<N. \<not>invset s0 ! i"
+  shows "i \<le> N \<Longrightarrow> \<forall>j<i. \<not>shrset (sendInv N i s0) ! j \<and> invset (sendInv N i s0) ! j = shrset s0 ! j"
+proof (induction i)
+  case 0
+  then show ?case by auto
+next
+  case (Suc i)
+  let ?s'="sendInv N i s0"
+  have a: "system_inv1 N (?s', clist)"
+    apply (rule sendInv_inv')
+    using assms(1) Suc(2) by auto
+  have b: ?case if "shrset ?s' ! i"
+  proof -
+    have b1: "sendInv N (Suc i) s0 = ?s'\<lparr>shrset := (shrset ?s')[i := False], invset := (invset ?s')[i := True]\<rparr>"
+      using that by (auto simp add: Let_def)
+    have b2: "i < length (shrset ?s')"
+      using Suc a by auto
+    have b3: "i < length (invset ?s')"
+      using Suc a by auto
+    show ?case
+      apply clarify subgoal for j
+        apply (cases "j = i")
+        subgoal unfolding b1 using b2 b3 apply auto
+          using assms(1) sendInv_shrset_same that by blast
+        subgoal
+          using b2 b3 Suc by (auto simp add: Let_def)
+        done
+      done
+  qed
+  have c: ?case if "\<not>shrset ?s' ! i"
+  proof -
+    have b1: "sendInv N (Suc i) s0 = ?s'"
+      using that by auto
+    show ?thesis
+      apply clarify subgoal for j
+        apply (cases "j = i")
+        apply (metis that assms Suc.prems b1 le_refl less_le_trans sendInv_shrset_same)
+        by (metis Suc.IH Suc.prems Suc_leD b1 less_antisym)
+      done
+  qed
+  show ?case
+    using b c by blast
+qed
+
+lemma set_curptr_sendInv_shrset:
+  assumes "system_inv1 N (s0, clist)"
+    and "\<forall>i<N. \<not>invset s0 ! i"
+    and "j < N"
+  shows "invset (set_curptr i b (sendInv N N s0)) ! j = shrset s0 ! j"
+        "\<not>shrset (set_curptr i b (sendInv N N s0)) ! j"
+proof -
+  have a: "invset (set_curptr i b (sendInv N N s0)) ! j = invset (sendInv N N s0) ! j"
+    by (auto simp add: set_curptr_def)
+  have a2: "shrset (set_curptr i b (sendInv N N s0)) ! j = shrset (sendInv N N s0) ! j"
+    by (auto simp add: set_curptr_def)
+  show "invset (set_curptr i b (sendInv N N s0)) ! j = shrset s0 ! j"
+    unfolding a using sendInv_shrset
+    by (meson assms order_refl)
+  show "\<not>shrset (set_curptr i b (sendInv N N s0)) ! j"
+    unfolding a2 using sendInv_shrset
+    by (metis assms order_refl)
+qed
+
+lemma grant_shrset_Some:
+  assumes "system_inv1 N (s0, clist)"
+    and "curptr s0 = Some i"
+  shows "j < N \<longrightarrow> invset (grant N s0) ! j = invset s0 ! j"
+        "j < N \<longrightarrow> j \<noteq> i \<longrightarrow> shrset (grant N s0) ! j = shrset s0 ! j"
+        "shrset (grant N s0) ! i \<longleftrightarrow> (shrset s0 ! i \<or> (\<forall>k<N. \<not>invset (grant N s0) ! k))"
+proof -
+  have *: "i < N"
+    using assms(1,2) by auto
+  show a: "j < N \<longrightarrow> invset (grant N s0) ! j = invset s0 ! j" for j
+    using assms(2) by (auto simp add: grant_def)
+  show b: "j < N \<longrightarrow> j \<noteq> i \<longrightarrow> shrset (grant N s0) ! j = shrset s0 ! j" for j
+    using assms(2) by (auto simp add: grant_def)
+  have c: "shrset (grant N s0) ! i \<longleftrightarrow> (shrset s0 ! i \<or> (\<forall>k<N. \<not>invset s0 ! k))"
+    using assms(1,2) * by (auto simp add: grant_def)
+  show "shrset (grant N s0) ! i \<longleftrightarrow> (shrset s0 ! i \<or> (\<forall>k<N. \<not>invset (grant N s0) ! k))"
+    unfolding c by (auto simp add: a)
+qed
+
+lemma grant_shrset_None:
+  assumes "system_inv1 N (s0, clist)"
+    and "\<forall>i<N. \<not>invset s0 ! i"
+    and "curptr s0 = None"
+  shows "j < N \<longrightarrow> invset (grant N s0) ! j = invset s0 ! j"
+        "j < N \<longrightarrow> shrset (grant N s0) ! j = shrset s0 ! j"
+  using assms by (auto simp add: grant_def)
+
+lemma grant_sendInv_shrset:
+  assumes "system_inv1 N (s0, clist)"
+    and "\<forall>i<N. \<not>invset s0 ! i"
+    and "i < N"
+  shows "j < N \<longrightarrow> invset (grant N (set_curptr i b (sendInv N N s0))) ! j = shrset s0 ! j"
+        "j < N \<longrightarrow> j \<noteq> i \<longrightarrow> \<not>shrset (grant N (set_curptr i b (sendInv N N s0))) ! j"
+        "if \<forall>k<N. \<not> invset (grant N (set_curptr i b (sendInv N N s0))) ! k
+         then shrset (grant N (set_curptr i b (sendInv N N s0))) ! i \<and>
+              curptr (grant N (set_curptr i b (sendInv N N s0))) = None
+         else \<not>shrset (grant N (set_curptr i b (sendInv N N s0))) ! i \<and>
+              curptr (grant N (set_curptr i b (sendInv N N s0))) = Some i"
+proof -
+  let ?s'="set_curptr i b (sendInv N N s0)"
+  have a1: "curptr ?s' = Some i"
+    by (auto simp add: set_curptr_def)
+  have a2: "system_inv1 N (?s', clist)"
+    apply (rule set_curptr_inv[OF assms(3)])
+    apply (rule sendInv_inv) by (rule assms(1))
+  have b1: "j < N \<longrightarrow> invset (grant N ?s') ! j = invset ?s' ! j"
+           "j < N \<longrightarrow> j \<noteq> i \<longrightarrow> shrset (grant N ?s') ! j = shrset ?s' ! j"
+    using grant_shrset_Some[OF a2 a1] by auto
+  show "j < N \<longrightarrow> invset (grant N ?s') ! j = shrset s0 ! j"
+    using b1(1) assms(1) assms(2) set_curptr_sendInv_shrset(1) by blast
+  show "j < N \<longrightarrow> j \<noteq> i \<longrightarrow> \<not>shrset (grant N ?s') ! j"
+    using assms(1) assms(2) b1(2) set_curptr_sendInv_shrset(2) by blast
+  show "if \<forall>k<N. \<not> invset (grant N ?s') ! k then
+          shrset (grant N ?s') ! i \<and> curptr (grant N ?s') = None
+        else
+          \<not>shrset (grant N ?s') ! i \<and> curptr (grant N ?s') = Some i"
+  proof -
+    have c1: "length (shrset (set_curptr i b (sendInv N N s0))) = N"
+      using a2 by auto
+    show ?thesis
+      apply (auto simp add: grant_def a1 c1 assms(3))
+      using set_curptr_sendInv_shrset(2)[OF assms(1,2,3)] by auto
+  qed
+qed
+
+\<comment> \<open>apply_grant does not change either invset or shrset\<close>
+lemma apply_grant_shrset:
+  "invset (fst (apply_grant N s1 p)) ! k = invset (fst p) ! k"
+  "shrset (fst (apply_grant N s1 p)) ! k = shrset (fst p) ! k"
+  "curptr (fst (apply_grant N s1 p)) = curptr (fst p)"
+  by (cases p, simp add: apply_grant.simps; cases "curptr s1", auto)+
+
+lemma sInv_shrset:
+  assumes "system_inv1 N (s, clist)"
+    and "i < N"
+    and "k < N"
+    and "if \<forall>j<N. \<not>invset s ! j then shrset s ! k \<and> curptr s = None
+         else \<not>shrset s ! k \<and> curptr s = Some k"
+    and "j < N \<longrightarrow> j \<noteq> k \<longrightarrow> \<not>shrset s ! j"
+  shows "j < N \<longrightarrow> j \<noteq> i \<longrightarrow> invset (fst (sInv N i (s, clist))) ! j = invset s ! j"
+        "\<not>invset (fst (sInv N i (s, clist))) ! i"
+        "j < N \<longrightarrow> j \<noteq> k \<longrightarrow> \<not>shrset (fst (sInv N i (s, clist))) ! j"
+        "if \<forall>j<N. \<not>invset (fst (sInv N i (s, clist))) ! j then
+           shrset (fst (sInv N i (s, clist))) ! k \<and> curptr (fst (sInv N i (s, clist))) = None
+         else
+           \<not>shrset (fst (sInv N i (s, clist))) ! k \<and> curptr (fst (sInv N i (s, clist))) = Some k"
+proof -
+  let ?s'="s\<lparr>invset := (invset s)[i := False]\<rparr>"
+  let ?clist'="clist[i := (clist ! i)\<lparr>st := Invalid\<rparr>]"
+  let ?s2="grant N ?s'"
+  let ?s3="apply_grant N ?s' (grant N ?s', ?clist')"
+  have c: "invset ?s2 ! j = invset ?s' ! j" for j
+    unfolding grant_def
+    apply (cases "curptr (s\<lparr>invset := (invset s)[i := False]\<rparr>)") by auto
+  have c2: "shrset ?s2 ! j = shrset s ! j" if "curptr s = None" for j
+    unfolding grant_def using that by auto
+  have c3: "j \<noteq> k \<longrightarrow> shrset ?s2 ! j = shrset s ! j" if "curptr s = Some k" for j
+    unfolding grant_def using that by auto
+  have d: "invset (fst ?s3) ! j = invset ?s2 ! j" for j
+    unfolding apply_grant.simps
+    apply (cases "curptr (s\<lparr>invset := (invset s)[i := False]\<rparr>)") by auto
+  have c4: "shrset ?s2 ! k" "curptr ?s2 = None"
+    if "curptr s = Some k" "(\<forall>j<N. \<not>invset (fst (sInv N i (s, clist))) ! j)"
+  proof -
+    have c41: "\<forall>j<N. \<not> invset (s\<lparr>invset := (invset s)[i := False]\<rparr>) ! j"
+      using that(2) unfolding sInv.simps sInvAck.simps Let_def d c by auto
+    show "shrset ?s2 ! k"
+      unfolding grant_def using that(1) c41 assms(1,3) by auto
+    show "curptr ?s2 = None"
+      unfolding grant_def using that(1) c41 assms(1,3) by auto
+  qed
+  have c5: "shrset ?s2 ! k \<and> curptr ?s2 = None"
+    if "\<forall>j<N. \<not>invset (fst (sInv N i (s, clist))) ! j" "\<forall>j<N. \<not>invset s ! j"
+    unfolding grant_def using assms(4) that(2) by auto
+  have c6: "shrset ?s2 ! k \<and> curptr ?s2 = None"
+    if "\<forall>j<N. \<not>invset (fst (sInv N i (s, clist))) ! j" "\<not>(\<forall>j<N. \<not>invset s ! j)"
+    by (simp add: assms(4) c4(1) c4(2) that(1) that(2))
+  have c7: "\<not>shrset ?s2 ! k \<and> curptr ?s2 = Some k"
+    if "\<not>(\<forall>j<N. \<not>invset (fst (sInv N i (s, clist))) ! j)"
+  proof -
+    have c71: "\<not>(\<forall>j<N. \<not>invset s ! j)"
+      using that apply (auto simp add: sInv.simps sInvAck.simps Let_def d c)
+      by (metis (full_types) assms(2) list_update_id)
+    have c72: "curptr (s\<lparr>invset := (invset s)[i := False]\<rparr>) = Some k"
+      using c71 assms(4) by auto
+    have c73: "\<not>(\<forall>j<N. \<not>(invset s)[i := False] ! j)"
+      using that by (auto simp add: sInv.simps sInvAck.simps Let_def d c)
+    have c74: "grant N (s\<lparr>invset := (invset s)[i := False]\<rparr>) = s\<lparr>invset := (invset s)[i := False]\<rparr>"
+      by (auto simp add: grant_def c72 c73)
+    show ?thesis
+      apply (auto simp add: c74) using c71 assms(4) by auto
+  qed
+  have d2: "shrset (fst ?s3) ! j = shrset ?s2 ! j" for j
+    unfolding apply_grant.simps
+    apply (cases "curptr (s\<lparr>invset := (invset s)[i := False]\<rparr>)") by auto
+  have d3: "curptr (fst ?s3) = curptr ?s2"
+    unfolding apply_grant.simps
+    apply (cases "curptr (s\<lparr>invset := (invset s)[i := False]\<rparr>)") by auto
+  have c8: "shrset (fst ?s3) ! k \<and> curptr (fst ?s3) = None"
+    if "\<forall>j<N. \<not>invset (fst (sInv N i (s, clist))) ! j"
+    unfolding d2 d3 using c5 c6 that by blast
+  have c9: "\<not>shrset (fst ?s3) ! k \<and> curptr (fst ?s3) = Some k"
+    if "\<not>(\<forall>j<N. \<not>invset (fst (sInv N i (s, clist))) ! j)"
+    unfolding d2 d3 using c7 that by blast
+  show "j < N \<longrightarrow> j \<noteq> i \<longrightarrow> invset (fst (sInv N i (s, clist))) ! j = invset s ! j"
+    by (auto simp add: sInv.simps sInvAck.simps Let_def d c)
+  show "\<not>invset (fst (sInv N i (s, clist))) ! i"
+    using assms by (auto simp add: sInv.simps sInvAck.simps Let_def d c)
+  show "j < N \<longrightarrow> j \<noteq> k \<longrightarrow> \<not>shrset (fst (sInv N i (s, clist))) ! j"
+    apply clarify unfolding sInv.simps sInvAck.simps Let_def d2
+    apply (cases "curptr s") apply (simp add: assms(5) c2)
+    by (metis assms(4) assms(5) c2 c3)
+  show "if \<forall>j<N. \<not>invset (fst (sInv N i (s, clist))) ! j then
+          shrset (fst (sInv N i (s, clist))) ! k \<and> curptr (fst (sInv N i (s, clist))) = None
+        else
+          \<not>shrset (fst (sInv N i (s, clist))) ! k \<and> curptr (fst (sInv N i (s, clist))) = Some k"
+    by (metis c8 c9 sInv.simps sInvAck.simps)
+qed
+
+lemma sInv_shrset':
+  assumes "system_inv1 N p"
+    and "i < N"
+    and "k < N"
+    and "if \<forall>j<N. \<not>invset (fst p) ! j then shrset (fst p) ! k \<and> curptr (fst p) = None
+         else \<not>shrset (fst p) ! k \<and> curptr (fst p) = Some k"
+    and "j < N \<longrightarrow> j \<noteq> k \<longrightarrow> \<not>shrset (fst p) ! j"
+  shows "j < N \<longrightarrow> j \<noteq> i \<longrightarrow> invset (fst (sInv N i p)) ! j = invset (fst p) ! j"
+        "\<not>invset (fst (sInv N i p)) ! i"
+        "j < N \<longrightarrow> j \<noteq> k \<longrightarrow> \<not>shrset (fst (sInv N i p)) ! j"
+        "if \<forall>j<N. \<not>invset (fst (sInv N i p)) ! j then
+           shrset (fst (sInv N i p)) ! k \<and> curptr (fst (sInv N i p)) = None
+         else
+           \<not>shrset (fst (sInv N i p)) ! k \<and> curptr (fst (sInv N i p)) = Some k"
+proof -
+  obtain a b where a: "fst p = a" "p = (a, b)"
+    by force
+  show "j < N \<longrightarrow> j \<noteq> i \<longrightarrow> invset (fst (sInv N i p)) ! j = invset (fst p) ! j"
+    unfolding a(1) unfolding a(2)
+    apply (rule sInv_shrset) using assms unfolding a(1) unfolding a(2) by auto
+  show "\<not>invset (fst (sInv N i p)) ! i"
+    unfolding a(1) unfolding a(2)
+    apply (rule sInv_shrset) using assms unfolding a(1) unfolding a(2) by auto
+  show "j < N \<longrightarrow> j \<noteq> k \<longrightarrow> \<not>shrset (fst (sInv N i p)) ! j"
+    unfolding a(1) unfolding a(2)
+    apply (rule sInv_shrset) using assms unfolding a(1) unfolding a(2) by auto
+  show "if \<forall>j<N. \<not>invset (fst (sInv N i p)) ! j then
+          shrset (fst (sInv N i p)) ! k \<and> curptr (fst (sInv N i p)) = None
+        else
+          \<not>shrset (fst (sInv N i p)) ! k \<and> curptr (fst (sInv N i p)) = Some k"
+    unfolding a(1) unfolding a(2)
+    apply (rule sInv_shrset) using assms unfolding a(1) unfolding a(2) by auto
+qed
+
+lemma apply_sendInv_shrset:
+  assumes "system_inv1 N (s2, clist)"
+    and "system_inv1 N (s0, clist)"
+    and "\<forall>i<N. invset s2 ! i = shrset s0 ! i"
+    and "k < N"
+    and "if \<forall>i<N. \<not>invset s2 ! i then shrset s2 ! k \<and> curptr s2 = None
+         else \<not>shrset s2 ! k \<and> curptr s2 = Some k"
+    and "\<forall>i<N. i \<noteq> k \<longrightarrow> \<not>shrset s2 ! i"
+  shows "j \<le> N \<Longrightarrow>
+    (i < j \<longrightarrow> \<not>invset (fst (apply_sendInv N j s0 (s2, clist))) ! i) \<and>
+    (i \<ge> j \<longrightarrow> i < N \<longrightarrow> invset (fst (apply_sendInv N j s0 (s2, clist))) ! i = shrset s0 ! i) \<and>
+    (i < N \<longrightarrow> i \<noteq> k \<longrightarrow> \<not>shrset (fst (apply_sendInv N j s0 (s2, clist))) ! i) \<and>
+    (if \<forall>i<N. \<not>invset (fst (apply_sendInv N j s0 (s2, clist))) ! i then
+       shrset (fst (apply_sendInv N j s0 (s2, clist))) ! k \<and> curptr (fst (apply_sendInv N j s0 (s2, clist))) = None
+     else
+       \<not>shrset (fst (apply_sendInv N j s0 (s2, clist))) ! k \<and> curptr (fst (apply_sendInv N j s0 (s2, clist))) = Some k)"
+proof (induction j)
+  case 0
+  show ?case
+    unfolding apply_sendInv.simps fst_conv
+    using assms by auto
+next
+  case (Suc j)
+  let ?s'="sendInv N j s0"
+  let ?s2="apply_sendInv N j s0 (s2, clist)"
+  have *: "j < N"
+    using Suc(2) by auto
+  have b: "system_inv1 N ?s2"
+    by (intro apply_sendInv_inv assms(1))
+  have b2: "i < j \<longrightarrow> \<not> invset (fst ?s2) ! i"
+    "j \<le> i \<longrightarrow> i < N \<longrightarrow> invset (fst ?s2) ! i = shrset s0 ! i"
+    "i < N \<longrightarrow> i \<noteq> k \<longrightarrow> \<not> shrset (fst ?s2) ! i"
+    "if \<forall>i<N. \<not> invset (fst ?s2) ! i then shrset (fst ?s2) ! k \<and> curptr (fst ?s2) = None
+     else \<not> shrset (fst ?s2) ! k \<and> curptr (fst ?s2) = Some k"
+    using Suc * by auto
+  have ?case if "shrset ?s' ! j"
+  proof -
+    have **: "shrset s0 ! j"
+      using sendInv_shrset_same[OF assms(2), where i=j and j=j] that by auto
+    have a: "apply_sendInv N (Suc j) s0 (s2, clist) = sInv N j ?s2"
+      unfolding apply_sendInv.simps Let_def using that by auto
+    have c: "i < N \<longrightarrow> i \<noteq> j \<longrightarrow> invset (fst (sInv N j ?s2)) ! i = invset (fst ?s2) ! i"
+      using sInv_shrset'(1)[OF b * assms(4) b2(4) b2(3)] by auto
+    have c2: "\<not> invset (fst (sInv N j ?s2)) ! j"
+      using sInv_shrset'(2)[OF b * assms(4) b2(4) b2(3)] by auto
+    have c3: "i < N \<longrightarrow> i \<noteq> k \<longrightarrow> \<not> shrset (fst (sInv N j ?s2)) ! i"
+      using sInv_shrset'(3)[OF b * assms(4) b2(4) b2(3)] by auto
+    have c4: "if \<forall>i<N. \<not> invset (fst (sInv N j ?s2)) ! i then
+                shrset (fst (sInv N j ?s2)) ! k \<and> curptr (fst (sInv N j ?s2)) = None
+              else
+                \<not>shrset (fst (sInv N j ?s2)) ! k \<and> curptr (fst (sInv N j ?s2)) = Some k"
+      using sInv_shrset'(4)[OF b * assms(4) b2(4) b2(3)] by auto
+    show ?case
+      apply (intro conjI)
+         apply (metis Suc.IH Suc.prems a c c2 le_def le_less_Suc_eq less_le_trans less_or_eq_imp_le)
+        apply (simp add: a b2(2) c)
+      using a c3 apply auto[1]
+      using a c4 by auto
+  qed
+  moreover have ?case if "\<not>shrset ?s' ! j"
+  proof -
+    have **: "\<not>shrset s0 ! j"
+      using sendInv_shrset_same[OF assms(2), where i=j and j=j] that by auto
+    have a: "apply_sendInv N (Suc j) s0 (s2, clist) = apply_sendInv N j s0 (s2, clist)"
+      unfolding apply_sendInv.simps Let_def using that by auto
+    show ?case
+      apply (rule conjI)
+       apply (metis "*" "**" Suc.IH a dual_order.strict_implies_order le_refl less_SucE)
+      using "*" Suc.IH Suc_leD a less_or_eq_imp_le by presburger
+  qed
+  ultimately show ?case
+    by blast
+qed
+
+lemma apply_sendInv_shrset':
+  assumes "system_inv1 N (s2, clist)"
+    and "system_inv1 N (s0, clist)"
+    and "\<forall>i<N. invset s2 ! i = shrset s0 ! i"
+    and "k < N"
+    and "if \<forall>i<N. \<not>invset s2 ! i then shrset s2 ! k \<and> curptr s2 = None
+         else \<not>shrset s2 ! k \<and> curptr s2 = Some k"
+    and "\<forall>i<N. i \<noteq> k \<longrightarrow> \<not>shrset s2 ! i"
+  shows "i < N \<Longrightarrow> \<not>invset (fst (apply_sendInv N N s0 (s2, clist))) ! i"
+    "i < N \<Longrightarrow> i \<noteq> k \<Longrightarrow> \<not>shrset (fst (apply_sendInv N N s0 (s2, clist))) ! i"
+    "if \<forall>i<N. \<not>invset (fst (apply_sendInv N N s0 (s2, clist))) ! i then
+       shrset (fst (apply_sendInv N N s0 (s2, clist))) ! k \<and> curptr (fst (apply_sendInv N N s0 (s2, clist))) = None
+     else
+       \<not>shrset (fst (apply_sendInv N N s0 (s2, clist))) ! k \<and> curptr (fst (apply_sendInv N N s0 (s2, clist))) = Some k"
+  using apply_sendInv_shrset[OF assms] by auto
+
+lemma sReq_shrset:
+  assumes "system_inv1 N (s0, clist)"
+    and "\<forall>i<N. \<not> invset s0 ! i"
+    and "i < N"
+  shows "k < N \<Longrightarrow> \<not>invset (fst (sReq N i b (s0, clist))) ! k"
+        "k < N \<Longrightarrow> k \<noteq> i \<Longrightarrow> \<not>shrset (fst (sReq N i b (s0, clist))) ! k"
+        "shrset (fst (sReq N i b (s0, clist))) ! i"
+        "curptr (fst (sReq N i b (s0, clist))) = None"
+proof -
+  let ?s'="grant N (set_curptr i b (sendInv N N s0))"
+  have a: "system_inv1 N (?s', clist)"
+    by (meson assms(1) assms(3) grant_inv sendInv_inv set_curptr_inv)
+  have b: "\<forall>k<N. invset ?s' ! k = shrset s0 ! k"
+    using assms grant_sendInv_shrset(1) by blast
+  have c: "if \<forall>k<N. \<not> invset ?s' ! k then shrset ?s' ! i \<and> curptr ?s' = None
+           else \<not> shrset ?s' ! i \<and> curptr ?s' = Some i"
+    using assms(1) assms(2) assms(3) grant_sendInv_shrset(3) by blast
+  have d: "\<forall>k<N. k \<noteq> i \<longrightarrow> \<not> shrset ?s' ! k"
+    by (meson assms(1) assms(2) assms(3) grant_sendInv_shrset(2))
+  have e: "k < N \<Longrightarrow> \<not> invset (fst (apply_sendInv N N s0 (?s', clist))) ! k"
+          "k < N \<Longrightarrow> k \<noteq> i \<Longrightarrow> \<not> shrset (fst (apply_sendInv N N s0 (?s', clist))) ! k" for k
+    using apply_sendInv_shrset'[OF a assms(1) b assms(3) c d] by auto
+  show "k < N \<Longrightarrow> \<not>invset (fst (sReq N i b (s0, clist))) ! k"
+    unfolding sReq.simps Let_def
+    apply (subst apply_grant_shrset) by (rule e(1))
+  show "k < N \<Longrightarrow> k \<noteq> i \<Longrightarrow> \<not>shrset (fst (sReq N i b (s0, clist))) ! k"
+    unfolding sReq.simps Let_def
+    apply (subst apply_grant_shrset) by (rule e(2))
+  show "shrset (fst (sReq N i b (s0, clist))) ! i"
+    unfolding sReq.simps Let_def
+    apply (subst apply_grant_shrset)
+    using a apply_sendInv_shrset'(3) assms(1) assms(3) b c d e(1) by presburger
+  show "curptr (fst (sReq N i b (s0, clist))) = None"
+    unfolding sReq.simps Let_def
+    apply (subst apply_grant_shrset)
+    using a apply_sendInv_shrset'(3) assms(1) assms(3) b c d e(1) by presburger
+qed
+
+lemma sReq_inv:
+  assumes "system_inv1 N (s0, clist)"
+    and "\<forall>i<N. \<not> invset s0 ! i"
+    and "i < N"
+  shows "system_inv1 N (sReq N i b (s0, clist))"
+proof -
+  let ?s1="set_curptr i b (sendInv N N s0)"
+  let ?s2="grant N ?s1"
+  let ?s3="apply_sendInv N N s0 (?s2, clist)"
+  have a: "curptr ?s1 = Some i"
+    unfolding set_curptr_def by auto
+  have b: "shrset (fst ?s3) ! i"
+    by (metis apply_grant_shrset(2) assms(1) assms(2) assms(3) sReq.simps sReq_shrset(3))
+  have c: "system_inv1 N ?s3"
+    by (intro apply_sendInv_inv grant_inv set_curptr_inv[OF assms(3)] sendInv_inv assms(1))
+  show ?thesis
+    apply (cases "apply_sendInv N N s0 (?s2, clist)") apply auto
+    apply (rule apply_grant_inv[where j=i])
+    using a b c by auto
+qed
+
+lemma sReqE_shrset:
+  assumes "system_inv1 N (s0, clist)"
+    and "\<forall>i<N. \<not> invset s0 ! i"
+    and "i < N"
+  shows "k < N \<Longrightarrow> \<not>invset (fst (sReqE N i (s0, clist))) ! k"
+        "k < N \<Longrightarrow> k \<noteq> i \<Longrightarrow> \<not>shrset (fst (sReqE N i (s0, clist))) ! k"
+        "shrset (fst (sReqE N i (s0, clist))) ! i"
+        "curptr (fst (sReqE N i (s0, clist))) = None"
+  unfolding sReqE.simps using sReq_shrset[OF assms] by auto
+
+lemma sReqE_inv1:
+  assumes "system_inv1 N (s0, clist)"
+    and "\<forall>i<N. \<not> invset s0 ! i"
+    and "i < N"
+  shows "system_inv1 N (sReqE N i (s0, clist))"
+  unfolding sReqE.simps using sReq_inv[OF assms] by auto
+
+lemma sReqS_shrset:
+  assumes "system_inv1 N (s0, clist)"
+    and "\<forall>i<N. \<not> invset s0 ! i"
+    and "i < N"
+  shows "k < N \<Longrightarrow> \<not>invset (fst (sReqS N i (s0, clist))) ! k"
+        "k < N \<Longrightarrow> k \<noteq> i \<Longrightarrow> shrset (fst (sReqS N i (s0, clist))) ! k = (if grantE s0 then False else shrset s0 ! k)"
+        "shrset (fst (sReqS N i (s0, clist))) ! i"
+  unfolding sReqS.simps
+  subgoal apply (cases "grantE s0")
+    using assms sReq_shrset(1) apply presburger
+    using assms by auto
+  subgoal apply (cases "grantE s0")
+    using assms sReq_shrset(2) apply presburger
+    using assms by auto
+  subgoal apply (cases "grantE s0")
+    using assms sReq_shrset(3) apply presburger
+    using assms by auto
+  done
+
+lemma sReqS_inv1:
+  assumes "system_inv1 N (s0, clist)"
+    and "\<forall>i<N. \<not> invset s0 ! i"
+    and "i < N"
+  shows "system_inv1 N (sReqS N i (s0, clist))"
+  unfolding sReqS.simps apply (cases "grantE s0")
+  subgoal unfolding if_P sReq.simps using sReq_inv[OF assms] by auto
+  subgoal unfolding if_not_P
+    using assms apply auto
+    subgoal for i' apply (cases "i = i'") by auto
+    subgoal for i' apply (cases "i = i'") by auto
+    done
+  done
+
+fun system_inv2 :: "nat \<Rightarrow> server \<times> client list \<Rightarrow> bool" where
+  "system_inv2 N (s0, clist) =
+    ((\<forall>i<N. \<not>invset s0 ! i) \<and>
+     (grantE s0 \<longrightarrow> (\<forall>i j. i < N \<longrightarrow> j < N \<longrightarrow> i \<noteq> j \<longrightarrow> \<not>shrset s0 ! i \<or> \<not>shrset s0 ! j)))"
+
+lemma sReqE_inv2:
+  assumes "system_inv1 N (s0, clist)"
+    and "system_inv2 N (s0, clist)"
+    and "i < N"
+  shows "system_inv2 N (sReqE N i (s0, clist))"
+proof -
+  let ?p="sReqE N i (s0, clist)"
+  have a: "\<forall>i<N. \<not>invset s0 ! i"
+    using assms(2) by auto
+  have b: "\<forall>i<N. \<not>invset (fst ?p) ! i"
+    using sReqE_shrset(1)[OF assms(1) a assms(3)] by auto
+  have c: "k < N \<Longrightarrow> k \<noteq> i \<Longrightarrow> \<not> shrset (fst ?p) ! k" for k
+    using sReqE_shrset(2)[OF assms(1) a assms(3)] by auto
+  show ?thesis
+    apply (cases "sReqE N i (s0, clist)")
+    using b c by auto
+qed
+
+lemma grant_grantE [simp]:
+  "grantE (grant N s) = grantE s"
+  apply (auto simp add: grant_def) apply (cases "curptr s") apply auto
+   apply (cases "\<forall>i<N. \<not> invset s ! i") apply auto
+  apply (cases "curptr s") by auto
+
+lemma apply_grant_grantE [simp]:
+  "grantE (fst (apply_grant N s1 p)) = grantE (fst p)"
+  apply (cases p) subgoal for s clist
+  apply (auto simp add: apply_grant.simps) apply (cases "curptr s1") apply auto
+   apply (cases "\<forall>i<N. \<not> invset s1 ! i") apply auto
+     apply (cases "grantE s1") apply auto apply (cases "curptr s1") by auto
+  done
+
+lemma sInvAck_grantE [simp]:
+  "grantE (fst (sInvAck N i (s, clist))) = grantE s"
+  by (auto simp add: sInvAck.simps Let_def)
+
+lemma sInv_grantE [simp]:
+  "grantE (fst (sInv N i p)) = grantE (fst p)"
+  apply (cases p) by (auto simp add: sInv.simps)
+
+lemma sReq_grantE:
+  "grantE (fst (sReq N i b (s0, clist))) = b"
+proof -
+  let ?s'="set_curptr i b (sendInv N N s0)"
+  let ?s2="grant N ?s'"
+  have a: "grantE ?s' = b"
+    unfolding set_curptr_def by auto
+  have b: "grantE ?s2 = b"
+    unfolding grant_def apply (cases "curptr ?s'") using a by auto
+  have c: "i \<le> N \<Longrightarrow> grantE (fst (apply_sendInv N i s0 (grant N ?s', clist))) = b" for i
+    apply (induction i) using b by (auto simp add: apply_sendInv.simps)
+  show ?thesis
+    unfolding sReq.simps Let_def using c by auto
+qed
+
+lemma sReqS_inv2:
+  assumes "system_inv1 N (s0, clist)"
+    and "system_inv2 N (s0, clist)"
+    and "i < N"
+  shows "system_inv2 N (sReqS N i (s0, clist))"
+proof -
+  let ?p="sReqS N i (s0, clist)"
+  have a: "\<forall>i<N. \<not>invset s0 ! i"
+    using assms(2) by auto
+  have b: "\<forall>i<N. \<not>invset (fst ?p) ! i"
+    using sReqS_shrset(1)[OF assms(1) a assms(3)] by auto
+  have c: "grantE s0 \<Longrightarrow> k < N \<Longrightarrow> k \<noteq> i \<Longrightarrow> \<not> shrset (fst ?p) ! k" for k
+    using sReqS_shrset(2)[OF assms(1) a assms(3)] by auto
+  have d: "\<not>grantE (fst ?p)"
+    unfolding sReqS.simps apply (cases "grantE s0") 
+    using sReq_grantE by auto
+  show ?thesis
+    apply (cases "sReqS N i (s0, clist)")
+    using b c d by auto
+qed
+
+subsection \<open>Overall result\<close>
+
+fun system_inv :: "nat \<Rightarrow> server \<times> client list \<Rightarrow> bool" where
+  "system_inv N (s, clist) \<longleftrightarrow>
+   system_inv1 N (s, clist) \<and> system_inv2 N (s, clist)"
+
+definition system_init :: "nat \<Rightarrow> server \<times> client list" where
+  "system_init N = (
+    \<lparr>invset = map (\<lambda>_. False) [0 ..< N],
+     shrset = map (\<lambda>_. False) [0 ..< N],
+     curptr = None, grantE = False\<rparr>,
+    map (\<lambda>_. \<lparr>st = Invalid\<rparr>) [0 ..< N])"
+
+lemma system_init_inv:
+  "system_inv N (system_init N)"
+  by (auto simp add: system_init_def)
+
+lemma sReqE_inv:
+  assumes "system_inv N (s0, clist)"
+    and "i < N"
+  shows "system_inv N (sReqE N i (s0, clist))"
+proof -
+  have a: "system_inv1 N (s0, clist)" "system_inv2 N (s0, clist)"
+    using assms(1) by auto
+  have b: "system_inv2 N (sReqE N i (s0, clist))"
+    apply (rule sReqE_inv2) using a assms(2) by auto
+  have c: "\<forall>i<N. \<not> invset s0 ! i"
+    using a by auto
+  have d: "system_inv1 N (sReqE N i (s0, clist))"
+    apply (rule sReqE_inv1) using a c assms(2) by auto
+  show ?thesis
+    by (metis b d system_inv.elims(3))
+qed
+
+lemma sReqS_inv:
+  assumes "system_inv N (s0, clist)"
+    and "i < N"
+  shows "system_inv N (sReqS N i (s0, clist))"
+proof -
+  have a: "system_inv1 N (s0, clist)" "system_inv2 N (s0, clist)"
+    using assms(1) by auto
+  have b: "system_inv2 N (sReqS N i (s0, clist))"
+    apply (rule sReqS_inv2) using a assms(2) by auto
+  have c: "\<forall>i<N. \<not> invset s0 ! i"
+    using a by auto
+  have d: "system_inv1 N (sReqS N i (s0, clist))"
+    apply (rule sReqS_inv1) using a c assms(2) by auto
+  show ?thesis
+    by (metis b d system_inv.elims(3))
+qed
+
+theorem sValidNF_ReqE_inv:
+  assumes "i < N"
+  shows
+  "sValidNF (system N)
+    (\<lambda>p es. system_inv N p \<and> nil\<^sub>e es)
+    (ReqE i)
+    (\<lambda>p es. system_inv N p \<and> nil\<^sub>e es)"
+  apply (rule sValidNF_weaken_pre[where P="\<lambda>p es. \<exists>s clist. system_inv N (s, clist) \<and> p = (s, clist) \<and> nil\<^sub>e es"])
+   apply auto[1]
+  apply (subst sValidNF_exists_pre2) apply clarify
+  apply (subst sValidNF_exists_pre2) apply clarify
+  apply (subst sValidNF_conj_pre) apply clarify
+  subgoal premises pre for s clist
+    apply (rule sValidNF_strengthen_post) prefer 2
+     apply (rule sValidNF_ReqE)
+    using sReqE_inv[OF pre assms(1)] by auto
+  done
+
+theorem sValidNF_ReqS_inv:
+  assumes "i < N"
+  shows
+  "sValidNF (system N)
+    (\<lambda>p es. system_inv N p \<and> nil\<^sub>e es)
+    (ReqS i)
+    (\<lambda>p es. system_inv N p \<and> nil\<^sub>e es)"
+  apply (rule sValidNF_weaken_pre[where P="\<lambda>p es. \<exists>s clist. system_inv N (s, clist) \<and> p = (s, clist) \<and> nil\<^sub>e es"])
+   apply auto[1]
+  apply (subst sValidNF_exists_pre2) apply clarify
+  apply (subst sValidNF_exists_pre2) apply clarify
+  apply (subst sValidNF_conj_pre) apply clarify
+  subgoal premises pre for s clist
+    apply (rule sValidNF_strengthen_post) prefer 2
+     apply (rule sValidNF_ReqS)
+    using sReqS_inv[OF pre assms(1)] by auto
+  done
+
+end
