Mapreduce.thy
@@ -1,0 +1,726 @@
+theory Mapreduce
+  imports EventSystem
+begin
+
+
+subsection \<open>Events\<close>
+
+datatype event =
+  QUERY "nat \<times> nat list"
+| RESPOND nat
+| TICK
+| INIT
+
+subsection \<open>Implementation of server\<close>
+
+record server =
+  input :: "nat list"
+  index :: nat
+  cursum :: nat
+  returned :: bool
+
+text \<open>Add a query\<close>
+definition query_impl :: "nat list \<Rightarrow> (server, event, unit) event_monad" where
+  "query_impl xs = put (\<lparr>input = xs, index = 0, cursum = 0, returned = False\<rparr>)"
+
+theorem query_impl_rule:
+  "\<lbrace> \<lambda>s es. s = s0 \<and> es = [] \<rbrace>
+     query_impl xs
+   \<lbrace> \<lambda>_ s es. s = \<lparr>input = xs, index = 0, cursum = 0, returned = False\<rparr> \<and> es = [] \<rbrace>!"
+  unfolding query_impl_def apply wp by auto
+
+text \<open>Implementation of tick: if there is a job present,
+  nondeterministically advance one index.\<close>
+definition tick_node_impl :: "(server, event, unit) event_monad" where
+  "tick_node_impl = (get \<bind> (\<lambda>s.
+   (if \<not>returned s then
+      if index s = length (input s) then
+        signal (RESPOND (cursum s)) \<bind> (\<lambda>_. put (s\<lparr>returned := True\<rparr>))
+      else
+        put (s\<lparr>index := index s + 1, cursum := cursum s + input s ! (index s)\<rparr>)
+    else
+      skip) \<squnion> skip))"
+
+definition tick_node_fun :: "server \<Rightarrow> server \<times> event list" where
+  "tick_node_fun s =
+    (if \<not>returned s then
+       if index s = length (input s) then
+         (s\<lparr>returned := True\<rparr>, [RESPOND (cursum s)])
+       else
+         (s\<lparr>index := index s + 1, cursum := cursum s + input s ! (index s)\<rparr>, [])
+     else
+       (s, []))"
+
+lemma tick_node_rule:
+  "\<lbrace> \<lambda>s es. s = s0 \<and> es = [] \<rbrace>
+     tick_node_impl
+   \<lbrace> \<lambda>_ s es. (s = fst (tick_node_fun s0) \<and> es = snd (tick_node_fun s0)) \<or>
+              (s = s0 \<and> es = []) \<rbrace>!"
+  unfolding tick_node_impl_def
+  apply (rule validNF_bind)
+   apply (rule validNF_get_post)
+  subgoal for s'
+    apply (subst validNF_conj_pre) apply (rule impI)
+    apply (rule validNF_nondet2)
+    subgoal apply wp by (auto simp add: tick_node_fun_def)
+    subgoal by wp
+    done
+  done
+
+fun node_inv :: "nat list \<times> bool \<Rightarrow> server \<Rightarrow> bool" where
+  "node_inv (xs, b) s = (
+    if b then returned s else
+    input s = xs \<and> index s \<le> length xs \<and> \<not>returned s \<and>
+    cursum s = sum (\<lambda>i. input s ! i) {0 ..< index s})"
+
+definition sum_list :: "nat list \<Rightarrow> nat" where
+  "sum_list xs = sum (\<lambda>i. xs ! i) {0 ..< length xs}"
+
+lemma tick_node_fun_inv:
+  assumes "node_inv (xs, False) s"
+  shows "(node_inv (xs, False) (fst (tick_node_fun s)) \<and> snd (tick_node_fun s) = []) \<or>
+         (node_inv (xs, True) (fst (tick_node_fun s)) \<and> snd (tick_node_fun s) = [RESPOND (sum_list xs)])"
+  using assms unfolding node_inv.simps tick_node_fun_def sum_list_def by auto
+
+lemma tick_node_rule2:
+  "node_inv (xs, False) s0 \<Longrightarrow>
+   \<lbrace> \<lambda>s es. s = s0 \<and> es = [] \<rbrace>
+     tick_node_impl
+   \<lbrace> \<lambda>_ s es. (node_inv (xs, False) s \<and> es = []) \<or>
+              (node_inv (xs, True) s \<and> es = [RESPOND (sum_list xs)]) \<rbrace>!"
+  apply (rule validNF_strengthen_post)
+   apply (rule tick_node_rule)
+  using tick_node_fun_inv by auto
+
+lemma tick_node_rule3:
+  "\<lbrace> \<lambda>s es. node_inv (xs, False) s \<and> es = [] \<rbrace>
+     tick_node_impl
+   \<lbrace> \<lambda>_ s es. (node_inv (xs, False) s \<and> es = []) \<or>
+              (node_inv (xs, True) s \<and> es = [RESPOND (sum_list xs)]) \<rbrace>!"
+  apply (rule validNF_weaken_pre[where Q="\<lambda>s es. \<exists>s0. node_inv (xs, False) s0 \<and> s = s0 \<and> es = []"])
+   apply (rule validNF_ex_pre)
+  subgoal for s0 apply (subst validNF_conj_pre)
+    using tick_node_rule2 by auto
+  by auto
+
+lemma tick_node_rule4:
+  "node_inv (xs, True) s0 \<Longrightarrow>
+   \<lbrace> \<lambda>s es. s = s0 \<and> es = [] \<rbrace>
+     tick_node_impl
+   \<lbrace> \<lambda>_ s es. node_inv (xs, True) s \<and> es = [] \<rbrace>!"
+  apply (rule validNF_strengthen_post)
+   apply (rule tick_node_rule)
+  by (auto simp add: tick_node_fun_def)
+
+lemma tick_node_rule5:
+  "\<lbrace> \<lambda>s es. node_inv (xs, True) s \<and> es = [] \<rbrace>
+     tick_node_impl
+   \<lbrace> \<lambda>_ s es. node_inv (xs, True) s \<and> es = [] \<rbrace>!"
+  apply (rule validNF_weaken_pre[where Q="\<lambda>s es. \<exists>s0. node_inv (xs, True) s0 \<and> s = s0 \<and> es = []"])
+  apply (rule validNF_ex_pre)
+  subgoal for s0 apply (subst validNF_conj_pre)
+    using tick_node_rule4 by auto
+  by auto
+
+lemma tick_node_rule6:
+  "\<lbrace> \<lambda>s es. node_inv (xs, b) s \<and> es = [] \<rbrace>
+     tick_node_impl
+   \<lbrace> \<lambda>_ s es. (node_inv (xs, b) s \<and> es = []) \<or> (b = False \<and> node_inv (xs, True) s \<and> es = [RESPOND (sum_list xs)]) \<rbrace>!"
+  apply (cases b)
+  using tick_node_rule3 tick_node_rule5 by auto
+
+record client =
+  num_received :: nat
+  acc :: nat
+  alldone :: bool
+
+text \<open>Implementation of respond\<close>
+definition respond_impl :: "nat \<Rightarrow> nat \<Rightarrow> (client, event, unit) event_monad" where
+  "respond_impl N a = (get \<bind> (\<lambda>s.
+    put (s\<lparr>acc := acc s + a, num_received := num_received s + 1\<rparr>)) \<bind> (\<lambda>_.
+    get \<bind> (\<lambda>s.
+    if num_received s = N then
+      put (s\<lparr>alldone := True\<rparr>)
+    else
+      skip)))"
+
+definition respond_fun :: "nat \<Rightarrow> nat \<Rightarrow> client \<Rightarrow> client" where
+  "respond_fun N a s = (let s' = s\<lparr>acc := acc s + a, num_received := num_received s + 1\<rparr> in
+                    if num_received s' = N then s'\<lparr>alldone := True\<rparr> else s')"
+
+theorem validNF_respond:
+  "\<lbrace> \<lambda>s es. s = s0 \<and> es = [] \<rbrace>
+     respond_impl N a
+   \<lbrace> \<lambda>_ s es. s = respond_fun N a s0 \<and> es = [] \<rbrace>!"
+  unfolding respond_impl_def
+  apply wp by (auto simp add: respond_fun_def)
+
+text \<open>Implementation of init\<close>
+definition init_impl :: "nat \<Rightarrow> nat list list \<Rightarrow> (client, event, unit) event_monad" where
+  "init_impl N data = (
+    whileLoop (\<lambda>i _. i < N)
+      (\<lambda>i. signal (QUERY (i, data ! i)) \<bind> (\<lambda>_.
+           return (Suc i))) 0) \<bind> (\<lambda>_. return ())"
+
+subsection \<open>Verify the event system\<close>
+
+definition tick_impl :: "nat \<Rightarrow> (server list \<times> client, event, unit) event_monad" where
+  "tick_impl N = (
+    whileLoop (\<lambda>i _. i < N)
+      (\<lambda>i. apply_fst (apply_idx tick_node_impl i) \<bind> (\<lambda>_.
+           return (Suc i))) 0) \<bind> (\<lambda>_. return ())"
+
+fun system :: "nat \<Rightarrow> nat list list \<Rightarrow> (event, server list \<times> client) event_system" where
+  "system N data (QUERY (i, xs)) = Some (apply_fst (apply_idx (query_impl xs) i))"
+| "system N data (RESPOND a) = Some (apply_snd (respond_impl N a))"
+| "system N data TICK = Some (tick_impl N)"
+| "system N data INIT = Some (apply_snd (init_impl N data))"
+
+definition server_inv :: "nat \<Rightarrow> nat list list \<Rightarrow> bool list \<Rightarrow> server list \<Rightarrow> bool" where
+  "server_inv N data bs ss =
+    (length bs = N \<and> length ss = N \<and>
+    (\<forall>i. i < N \<longrightarrow> node_inv (data ! i, bs ! i) (ss ! i)))"
+
+fun tick_events :: "nat \<Rightarrow> bool list \<Rightarrow> bool list \<Rightarrow> nat list list \<Rightarrow> nat \<Rightarrow> event list" where
+  "tick_events N bs bs' xss 0 = []"
+| "tick_events N bs bs' xss (Suc i) =
+    (if \<not>bs ! i \<and> bs' ! i then tick_events N bs bs' xss i @ [RESPOND (sum_list (xss ! i))]
+     else tick_events N bs bs' xss i)"
+
+lemma tick_events_cong:
+  "\<forall>i<r. bs1 ! i = bs2 ! i \<Longrightarrow> tick_events N bs bs1 xss r = tick_events N bs bs2 xss r"
+  apply (induction r) by auto
+
+definition dominates :: "nat \<Rightarrow> bool list \<Rightarrow> bool list \<Rightarrow> bool" where
+  "dominates N bs bs' = (\<forall>i<N. bs ! i \<longrightarrow> bs' ! i)"
+
+lemma tick_rule:
+  "\<lbrace> \<lambda>p es. server_inv N xss bs (fst p) \<and> snd p = c0 \<and> nil\<^sub>e es \<rbrace>
+     tick_impl N
+   \<lbrace> \<lambda>_ p es. \<exists>bs'. server_inv N xss bs' (fst p) \<and> dominates N bs bs' \<and> snd p = c0 \<and> es = tick_events N bs bs' xss N \<rbrace>!"
+  unfolding tick_impl_def
+  apply (rule validNF_bind) prefer 2 apply (rule validNF_return)
+  apply (rule validNF_whileLoop[where
+        I="\<lambda>i p es. i \<le> N \<and> (\<exists>bs'. server_inv N xss bs' (fst p) \<and>
+              length bs' = N \<and> dominates N bs bs' \<and> (\<forall>j\<ge>i. bs ! j = bs' ! j) \<and>
+              snd p = c0 \<and> es = tick_events N bs bs' xss i)" and
+        R="measure (\<lambda>(i,p). (N - i))"])
+  subgoal for p es
+    apply (rule conjI) apply simp
+    apply (rule exI[where x=bs])
+    by (auto simp add: nil_event_def server_inv_def dominates_def)
+  subgoal for r s
+    apply (rule validNF_bind) prefer 2
+     apply (rule validNF_return)
+    apply (rule validNF_weaken_pre[where
+          Q="\<lambda>p es. r < N \<and> (\<exists>bs'. (length bs' = N \<and> dominates N bs bs' \<and>
+                (\<forall>i\<ge>r. bs ! i = bs' ! i)) \<and>
+                (server_inv N xss bs' (fst p) \<and> es = tick_events N bs bs' xss r) \<and> snd p = c0)"])
+     prefer 2 subgoal by auto
+    apply (subst validNF_conj_pre) apply (rule impI)
+    apply (rule validNF_ex_pre) subgoal premises pre for bs'
+      apply (subst validNF_conj_pre) apply (rule impI)
+      apply (subst server_inv_def)
+      apply (rule validNF_strengthen_post)
+       apply (rule validNF_apply_fst)
+       apply (rule validNF_frame)
+       apply (rule validNF_weaken_pre[where
+            Q="\<lambda>p es. length p = N \<and> (\<forall>i. i < N \<longrightarrow> node_inv (xss ! i, bs' ! i) (p ! i)) \<and> nil\<^sub>e es"])
+        prefer 2 subgoal by (auto simp add: nil_event_def)
+       apply (rule validNF_apply_idx2)
+      unfolding nil_event_def apply (rule tick_node_rule6)
+      apply (rule pre)
+      subgoal for r' s' es'
+        unfolding chop_event_def apply clarify subgoal for es1 es2
+          apply (elim disjE)
+          subgoal
+            apply (intro conjI)
+            subgoal using pre by auto
+            subgoal apply (rule exI[where x=bs'])
+              by (auto simp add: server_inv_def)
+            subgoal using pre by auto
+            done
+          subgoal
+            apply (intro conjI)
+            subgoal using pre by auto
+            subgoal apply (rule exI[where x="bs'[r := True]"])
+              apply (intro conjI)
+              subgoal unfolding server_inv_def
+                apply (rule conjI) apply simp
+                apply clarify subgoal for i apply (cases "i = r")
+                  subgoal by auto
+                  subgoal by auto
+                  done
+                done
+              subgoal by auto
+              subgoal by (metis dominates_def nth_list_update pre)
+              subgoal by auto
+              subgoal by auto
+              subgoal unfolding tick_events.simps
+                using pre by (auto simp add: tick_events_cong)
+              done
+            subgoal using pre by auto
+            done
+          done
+        done
+      done
+    done
+  subgoal by auto
+  subgoal by auto
+  done
+
+lemma sValidNF_Respond:
+  "sValidNF (system N data)
+    (\<lambda>p es. P (fst p) \<and> snd p = c \<and> nil\<^sub>e es)
+    (RESPOND a)
+    (\<lambda>p es. P (fst p) \<and> snd p = respond_fun N a c \<and> nil\<^sub>e es)"
+  apply (rule sValidNF_weaken_pre[where P="\<lambda>p es. (P (fst p) \<and> snd p = c) \<and> nil\<^sub>e es"])
+  apply simp
+  apply (rule sValidNF_Some)
+  apply (rule system.simps)
+  apply (rule validNF_weaken_pre)
+  apply (rule validNF_apply_snd[where R="\<lambda>s. P s"])
+    apply (rule validNF_respond)
+   apply (auto simp add: nil_event_def)
+  apply (rule sValidNF_list_strengthen_post)
+  prefer 2 
+   apply (rule sValidNF_list_null)
+  by auto
+
+fun sum_tick_events :: "nat \<Rightarrow> bool list \<Rightarrow> bool list \<Rightarrow> nat list list \<Rightarrow> nat \<Rightarrow> nat" where
+  "sum_tick_events N bs bs' xss 0 = 0"
+| "sum_tick_events N bs bs' xss (Suc i) =
+    (if \<not>bs ! i \<and> bs' ! i then sum_tick_events N bs bs' xss i + sum_list (xss ! i)
+     else sum_tick_events N bs bs' xss i)"
+
+fun count_tick_events :: "nat \<Rightarrow> bool list \<Rightarrow> bool list \<Rightarrow> nat list list \<Rightarrow> nat \<Rightarrow> nat" where
+  "count_tick_events N bs bs' xss 0 = 0"
+| "count_tick_events N bs bs' xss (Suc i) =
+    (if \<not>bs ! i \<and> bs' ! i then count_tick_events N bs bs' xss i + 1
+     else count_tick_events N bs bs' xss i)"
+
+lemma sValidNF_Respond_tick_events:
+  assumes "num_received c \<ge> N \<longleftrightarrow> alldone c"
+  shows
+  "sValidNF_list (system N data)
+    (\<lambda>p es. P (fst p) \<and> snd p = c \<and> nil\<^sub>e es)
+    (tick_events N bs bs' data i)
+    (\<lambda>p es. P (fst p) \<and> snd p = c\<lparr>acc := acc c + sum_tick_events N bs bs' data i,
+         num_received := num_received c + count_tick_events N bs bs' data i,
+         alldone := alldone c \<or> (\<exists>i'\<le>i. num_received c + count_tick_events N bs bs' data i' = N)\<rparr> \<and> nil\<^sub>e es)"
+proof (induction i)
+  case 0
+  then show ?case 
+    apply auto
+    apply (rule sValidNF_list_strengthen_post) prefer 2
+     apply (rule sValidNF_list_null)
+    using assms by auto
+next
+  case (Suc i)
+  show ?case
+    apply (cases "\<not>bs ! i \<and> bs' ! i")
+    subgoal apply auto
+      apply (rule sValidNF_list_append)
+       apply (rule Suc)
+      apply (rule sValidNF_list_single)
+      apply (rule sValidNF_strengthen_post)
+      prefer 2
+      apply (rule sValidNF_Respond)
+      apply (auto simp add: respond_fun_def Let_def)
+      subgoal premises pre for es
+      proof -
+        have "num_received c + count_tick_events N bs bs' data (Suc i) = N"
+          using pre by auto
+        then have "\<exists>i'\<le>Suc i. num_received c + count_tick_events N bs bs' data i' = N"
+          by auto
+        then show ?thesis
+          by auto
+      qed
+      subgoal premises pre for es
+      proof -
+        have "num_received c + count_tick_events N bs bs' data (Suc i) \<noteq> N"
+          using pre by auto
+        then have "(\<exists>i'\<le>i. num_received c + count_tick_events N bs bs' data i' = N) \<longleftrightarrow>
+                   (\<exists>i'\<le>Suc i. num_received c + count_tick_events N bs bs' data i' = N)"
+          using le_Suc_eq by blast
+        then show ?thesis
+          by auto
+      qed
+      done
+    subgoal premises pre
+    proof -
+      have "count_tick_events N bs bs' data (Suc i) = count_tick_events N bs bs' data i"
+        using pre by auto
+      then have a: "(\<exists>i'\<le>i. num_received c + count_tick_events N bs bs' data i' = N) \<longleftrightarrow>
+                 (\<exists>i'\<le>Suc i. num_received c + count_tick_events N bs bs' data i' = N)"
+        by (metis le_Suc_eq pl_pl_rels)
+      show ?thesis
+        apply (auto simp add: pre)
+        apply (rule sValidNF_list_strengthen_post)
+         prefer 2 apply (rule Suc)
+        using a by auto
+    qed
+    done
+qed
+
+lemma sValidNF_Tick:
+  assumes "num_received c0 \<ge> N \<longleftrightarrow> alldone c0"
+  shows
+  "sValidNF (system N data)
+    (\<lambda>p es. server_inv N data bs (fst p) \<and> snd p = c0 \<and> nil\<^sub>e es)
+    TICK
+    (\<lambda>p es. \<exists>bs'. server_inv N data bs' (fst p) \<and> dominates N bs bs' \<and>
+        snd p = c0\<lparr>acc := acc c0 + sum_tick_events N bs bs' data N,
+                   num_received := num_received c0 + count_tick_events N bs bs' data N,
+                   alldone := alldone c0 \<or> (\<exists>i'\<le>N. num_received c0 + count_tick_events N bs bs' data i' = N)\<rparr> \<and> nil\<^sub>e es)"
+  apply (rule sValidNF_weaken_pre[where P="\<lambda>p es. (server_inv N data bs (fst p) \<and> snd p = c0) \<and> nil\<^sub>e es"])
+  apply simp
+  apply (rule sValidNF_Some)
+  apply (rule system.simps)
+   apply (subst conj_assoc)
+  apply (rule tick_rule)
+  subgoal for p es
+    apply clarify subgoal for bs'
+      apply (rule sValidNF_list_strengthen_post) prefer 2
+       apply (rule sValidNF_list_weaken_pre[where P="\<lambda>p es. server_inv N data bs' (fst p) \<and> snd p = c0 \<and> nil\<^sub>e es"])
+      apply auto[1]
+      apply (rule sValidNF_Respond_tick_events[OF assms])
+      subgoal for p' es'
+        apply (rule exI[where x=bs'])
+        by auto
+      done
+    done
+  done
+
+fun system_inv :: "nat \<Rightarrow> nat list list \<Rightarrow> server list \<times> client \<Rightarrow> bool" where
+  "system_inv N data (ss, c) =
+    (\<exists>bs. server_inv N data bs ss \<and>
+          num_received c = sum (\<lambda>i. if bs ! i then 1 else 0) {0 ..< N} \<and>
+          acc c = sum (\<lambda>i. if bs ! i then sum_list (data ! i) else 0) {0 ..< N} \<and>
+          alldone c = (num_received c \<ge> N))"
+
+lemma dominates_num_received':
+  assumes "dominates N bs bs'"
+  shows
+    "k \<le> N \<Longrightarrow>
+     sum (\<lambda>i. if bs ! i then 1 else 0) {0 ..< k} + count_tick_events N bs bs' data k =
+     sum (\<lambda>i. if bs' ! i then 1 else 0) {0 ..< k}"
+proof (induction k)
+  case 0
+  then show ?case by auto
+next
+  case (Suc k)
+  show ?case
+    apply auto
+    subgoal using Suc by auto
+    subgoal using Suc by auto
+    subgoal using assms(1) unfolding dominates_def
+      using Suc by simp
+    done
+qed
+
+lemma dominates_num_received:
+  "dominates N bs bs' \<Longrightarrow>
+   sum (\<lambda>i. if bs ! i then 1 else 0) {0 ..< N} + count_tick_events N bs bs' data N =
+   sum (\<lambda>i. if bs' ! i then 1 else 0) {0 ..< N}"
+  using dominates_num_received' by auto
+
+lemma dominates_acc':
+  assumes "dominates N bs bs'"
+  shows
+    "k \<le> N \<Longrightarrow>
+      sum (\<lambda>i. if bs ! i then sum_list (data ! i) else 0) {0 ..< k} + sum_tick_events N bs bs' data k =
+      sum (\<lambda>i. if bs' ! i then sum_list (data ! i) else 0) {0 ..< k}"
+proof (induction k)
+  case 0
+  then show ?case by auto
+next
+  case (Suc k)
+  show ?case
+    apply auto
+    subgoal using Suc by auto
+    subgoal using Suc by auto
+    subgoal using assms(1) unfolding dominates_def
+      using Suc by simp
+    done
+qed
+
+lemma dominates_acc:
+  "dominates N bs bs' \<Longrightarrow>
+   sum (\<lambda>i. if bs ! i then sum_list (data ! i) else 0) {0 ..< N} + sum_tick_events N bs bs' data N =
+   sum (\<lambda>i. if bs' ! i then sum_list (data ! i) else 0) {0 ..< N}"
+  using dominates_acc' by auto
+
+lemma count_tick_events_mono:
+  "count_tick_events N bs bs' data i \<le> count_tick_events N bs bs' data (a + i)"
+  apply (induction a) by auto 
+
+lemma count_tick_events_mono2:
+  "i \<le> j \<Longrightarrow> count_tick_events N bs bs' data i \<le> count_tick_events N bs bs' data j"
+  using count_tick_events_mono
+  by (metis add.commute nat_le_iff_add)
+
+lemma count_tick_events_dense:
+  "a \<le> count_tick_events N bs bs' data j \<Longrightarrow> \<exists>i\<le>j. a = count_tick_events N bs bs' data i"
+proof (induction j)
+  case 0
+  then show ?case by auto
+next
+  case (Suc j)
+  have "a \<le> count_tick_events N bs bs' data j + 1"
+    using Suc(2) apply (cases "\<not> bs ! j \<and> bs' ! j") by auto
+  have "a \<le> count_tick_events N bs bs' data j + 1"
+    using Suc(2) apply (cases "\<not> bs ! j \<and> bs' ! j") by auto
+  then have "a = count_tick_events N bs bs' data j + 1 \<or> a \<le> count_tick_events N bs bs' data j"
+    by auto
+  then show ?case
+    apply (elim disjE)
+    subgoal apply (rule exI[where x="Suc j"])
+      by (metis Suc.prems add_diff_cancel_left' add_le_cancel_right count_tick_events.simps(2)
+                diff_is_0_eq' le_numeral_extra(4) plus_1_eq_Suc zero_neq_one)
+    subgoal using Suc(1)
+      by (meson le_SucI)
+    done
+qed
+
+lemma count_tick_events_dense2:
+  assumes "N > num_received c0"
+    and "N \<le> num_received c0 + count_tick_events N bs bs' data N"
+  shows "\<exists>i\<le>N. N = num_received c0 + count_tick_events N bs bs' data i"
+proof -
+  have a: "N - num_received c0 \<le> count_tick_events N bs bs' data N"
+    using assms by auto
+  then obtain i where b: "i \<le> N" "N - num_received c0 = count_tick_events N bs bs' data i"
+    using count_tick_events_dense by blast
+  then have c: "N = num_received c0 + count_tick_events N bs bs' data i"
+    using assms by auto
+  show ?thesis
+    using b c by auto
+qed
+
+lemma count_tick_events_incr:
+  "(N \<le> num_received c0 \<or> (\<exists>i'\<le>N. num_received c0 + count_tick_events N bs bs' data i' = N)) \<longleftrightarrow>
+   (N \<le> num_received c0 + count_tick_events N bs bs' data N)"
+  apply (rule iffI, elim disjE)
+  subgoal by auto
+  subgoal using count_tick_events_mono2
+    by (metis add_left_mono)
+  subgoal using count_tick_events_dense2
+    by (metis not_le_imp_less)
+  done
+
+lemma sValidNF_Tick2:
+  "sValidNF (system N data)
+    (\<lambda>p es. system_inv N data p \<and> nil\<^sub>e es)
+    TICK
+    (\<lambda>p es. system_inv N data p \<and> nil\<^sub>e es)"
+  apply (rule sValidNF_weaken_pre[where
+        P="\<lambda>p es. \<exists>bs c0. (num_received c0 \<ge> N \<longleftrightarrow> alldone c0) \<and>
+            num_received c0 = sum (\<lambda>i. if bs ! i then 1 else 0) {0 ..< N} \<and>
+            acc c0 = sum (\<lambda>i. if bs ! i then sum_list (data ! i) else 0) {0 ..< N} \<and>
+            server_inv N data bs (fst p) \<and>
+            snd p = c0 \<and> nil\<^sub>e es"])
+  subgoal for p es
+    apply (cases p) by auto
+  apply (subst sValidNF_exists_pre2) apply (rule allI)
+  apply (subst sValidNF_exists_pre2) apply (rule allI)
+  apply (subst sValidNF_conj_pre) apply (rule impI)
+  apply (subst sValidNF_conj_pre) apply (rule impI)
+  apply (subst sValidNF_conj_pre) apply (rule impI)
+  subgoal premises pre for bs c0
+    apply (rule sValidNF_strengthen_post) prefer 2
+     apply (rule sValidNF_Tick[OF pre(1)])
+    subgoal for p es
+      apply (cases p) subgoal for ss c
+        apply clarify subgoal for bs'
+          unfolding system_inv.simps
+          apply (rule exI[where x=bs'])
+          apply (intro conjI)
+          subgoal by auto
+          subgoal apply (auto simp add: pre(2))
+            apply (rule dominates_num_received) by auto
+          subgoal apply (auto simp add: pre(3))
+            apply (rule dominates_acc) by auto
+          subgoal apply simp
+            using pre(1) count_tick_events_incr by blast
+          done
+        done
+      done
+    done
+  done
+
+subsection \<open>Final results\<close>
+
+theorem validNF_init:
+  "\<lbrace> \<lambda>c es. c = c0 \<and> es = [] \<rbrace>
+     init_impl N data
+   \<lbrace> \<lambda>_ c es. c = c0 \<and> es = map (\<lambda>i. QUERY (i, data ! i)) [0 ..< N] \<rbrace>!"
+  unfolding init_impl_def
+  apply (rule validNF_bind) prefer 2
+   apply (rule validNF_return)
+  apply (rule validNF_whileLoop[where I="\<lambda>r c es. c = c0 \<and> r \<le> N \<and> es = map (\<lambda>i. QUERY (i, data ! i)) [0 ..< r]" and
+                                      R="measure (\<lambda>(r,c). (N - r))"])
+  subgoal for c es by auto
+  subgoal for r s apply wp by auto
+  subgoal by auto
+  subgoal for r s es by auto
+  done
+
+theorem sValidNF_Query:
+  "sValidNF (system N data)
+    (\<lambda>p es. p = (ss, c0) \<and> nil\<^sub>e es)
+    (QUERY (i, data ! i))
+    (\<lambda>p es. p = (ss[i := \<lparr>input = data ! i, index = 0, cursum = 0, returned = False\<rparr>], c0) \<and> nil\<^sub>e es)"
+  apply (rule sValidNF_Some)
+    apply (rule system.simps)
+  apply (rule validNF_weaken_pre)
+    apply (rule validNF_apply_fst[where R="\<lambda>s. s = c0"])
+    apply (rule validNF_apply_idx[OF query_impl_rule])
+  apply (auto simp add: nil_event_def)[1]
+  apply auto by (rule sValidNF_list_null)
+
+theorem sValidNF_list_queries:
+  assumes "length ss = N"
+  shows
+  "j \<le> N \<Longrightarrow>
+   sValidNF_list (system N data)
+    (\<lambda>p es. p = (ss, c0) \<and> nil\<^sub>e es)
+      (map (\<lambda>i. QUERY (i, data ! i)) [0..<j])
+    (\<lambda>p es. p = (map (\<lambda>i. if i < j then \<lparr>input = data ! i, index = 0, cursum = 0, returned = False\<rparr>
+                          else ss ! i) [0..<N], c0) \<and> nil\<^sub>e es)"
+proof (induction j)
+  case 0
+  then show ?case
+    using assms apply (auto simp add: map_nth)
+    by (rule sValidNF_list_null)
+next
+  case (Suc j)
+  have a: "map (\<lambda>i. QUERY (i, data ! i)) [0..<Suc j] = map (\<lambda>i. QUERY (i, data ! i)) [0..<j] @ [QUERY (j, data ! j)]"
+    by auto
+  have b: "sValidNF_list (system N data) (\<lambda>p es. p = (ss, c0) \<and> nil\<^sub>e es) (map (\<lambda>i. QUERY (i, data ! i)) [0..<j])
+   (\<lambda>p es. p = (map (\<lambda>i. if i < j then \<lparr>input = data ! i, index = 0, cursum = 0, returned = False\<rparr> else ss ! i) [0..<N], c0) \<and>
+          nil\<^sub>e es)"
+    using Suc by auto
+  show ?case
+    unfolding a apply (rule sValidNF_list_append)
+     apply (rule b)
+    apply (rule sValidNF_list_single)
+    apply (rule sValidNF_strengthen_post) prefer 2
+     apply (rule sValidNF_Query)
+    apply auto
+    apply (rule nth_equalityI)
+     apply auto subgoal for es i
+      apply (cases "i = j") by auto
+    done
+qed
+
+theorem sValidNF_list_queries':
+  assumes "length ss = N"
+  shows
+  "sValidNF_list (system N data)
+    (\<lambda>p es. p = (ss, c0) \<and> nil\<^sub>e es)
+    (map (\<lambda>i. QUERY (i, data ! i)) [0..<N])
+    (\<lambda>p es. p = (map (\<lambda>i. \<lparr>input = data ! i, index = 0, cursum = 0, returned = False\<rparr>) [0..<N], c0) \<and> nil\<^sub>e es)"
+proof -
+  have a: "sValidNF_list (system N data)
+    (\<lambda>p es. p = (ss, c0) \<and> nil\<^sub>e es)
+      (map (\<lambda>i. QUERY (i, data ! i)) [0..<N])
+    (\<lambda>p es. p = (map (\<lambda>i. if i < N then \<lparr>input = data ! i, index = 0, cursum = 0, returned = False\<rparr>
+                          else ss ! i) [0..<N], c0) \<and> nil\<^sub>e es)"
+    using sValidNF_list_queries[OF assms, where j=N] by auto
+  have b: "map (\<lambda>i. if i < N then \<lparr>input = data ! i, index = 0, cursum = 0, returned = False\<rparr>
+                    else ss ! i) [0..<N] = map (\<lambda>i. \<lparr>input = data ! i, index = 0, cursum = 0, returned = False\<rparr>) [0 ..< N]"
+    apply (rule nth_equalityI)
+    by auto
+  show ?thesis
+    using a b by auto
+qed
+
+fun init_state :: "nat \<Rightarrow> server list \<times> client \<Rightarrow> bool" where
+  "init_state N (ss, c) \<longleftrightarrow> length ss = N \<and> c = \<lparr>num_received = 0, acc = 0, alldone = False\<rparr>"
+
+theorem sValidNF_init:
+  assumes "length ss = N"
+  shows
+  "sValidNF (system N data)
+    (\<lambda>p es. p = (ss, c0) \<and> nil\<^sub>e es)
+     INIT
+    (\<lambda>p es. p = (map (\<lambda>i. \<lparr>input = data ! i, index = 0, cursum = 0, returned = False\<rparr>) [0 ..< N], c0) \<and> nil\<^sub>e es)"
+  apply (rule sValidNF_Some)
+    apply (rule system.simps)
+  apply (rule validNF_weaken_pre)
+    apply (rule validNF_apply_snd[where R="\<lambda>s. s = ss"])
+    apply (rule validNF_init)
+   apply (auto simp add: nil_event_def)
+  using sValidNF_list_queries'[OF assms] unfolding nil_event_def by auto
+
+theorem sValidNF_init_inv:
+  assumes "N > 0"
+  shows
+  "sValidNF (system N data)
+    (\<lambda>p es. init_state N p \<and> nil\<^sub>e es)
+     INIT
+    (\<lambda>p es. system_inv N data p \<and> nil\<^sub>e es)"
+  apply (rule sValidNF_weaken_pre[where P="\<lambda>p es. \<exists>ss c. init_state N (ss, c) \<and> p = (ss, c) \<and> nil\<^sub>e es"])
+   apply auto[1]
+  apply (subst sValidNF_exists_pre2) apply clarify
+  apply (subst sValidNF_exists_pre2) apply clarify
+  apply (subst sValidNF_conj_pre) apply clarify
+  subgoal premises pre for ss c
+    apply (rule sValidNF_strengthen_post)
+     prefer 2 apply (rule sValidNF_init)
+    using pre apply auto[1]
+    subgoal for p es
+      apply auto apply (rule exI[where x="map (\<lambda>i. False) [0..<N]"])
+      using pre assms by (auto simp add: server_inv_def)
+    done
+  done
+
+theorem system_inv_sum:
+  assumes "system_inv N data (ss, c)"
+    and "alldone c"
+  shows "acc c = sum (\<lambda>i. sum_list (data ! i)) {0 ..< N}"
+proof -
+  obtain bs where a: "server_inv N data bs ss"
+    "num_received c = sum (\<lambda>i. if bs ! i then 1 else 0) {0 ..< N}"
+    "acc c = sum (\<lambda>i. if bs ! i then sum_list (data ! i) else 0) {0 ..< N}"
+    "alldone c = (num_received c \<ge> N)"
+    using assms by auto
+  have b: "(\<forall>i<j. bs ! i) \<longleftrightarrow> sum (\<lambda>i. if bs ! i then 1 else 0) {0 ..< j} \<ge> j" for j
+    apply (induction j)
+    apply auto using not_less_less_Suc_eq by auto
+  have c: "\<forall>i<N. bs ! i"
+    using a(2,4) assms(2) b by auto
+  show ?thesis
+    using a(3) c by auto
+qed
+
+theorem system_inv_all':
+  assumes "N > 0"
+  shows
+  "sValidNF_list (system N data)
+    (\<lambda>p es. init_state N p \<and> nil\<^sub>e es)
+    (INIT # replicate n TICK)
+    (\<lambda>p es. system_inv N data p \<and> nil\<^sub>e es)"
+  apply (rule sValidNF_list_cons)
+  apply (rule sValidNF_init_inv[OF assms])
+  apply (induction n)
+  subgoal apply auto by (rule sValidNF_list_null)
+  subgoal for n
+    apply auto apply (rule sValidNF_list_cons)
+     apply (rule sValidNF_Tick2)
+    by auto
+  done
+
+theorem system_inv_all:
+  assumes "N > 0"
+  shows
+  "sValidNF_list (system N data)
+    (\<lambda>p es. init_state N p \<and> nil\<^sub>e es)
+    (INIT # replicate n TICK)
+    (\<lambda>p es. (alldone (snd p) \<longrightarrow> acc (snd p) = sum (\<lambda>i. sum_list (data ! i)) {0 ..< N}) \<and> nil\<^sub>e es)"
+  apply (rule sValidNF_list_strengthen_post)
+  prefer 2 apply (rule system_inv_all'[OF assms])
+  using system_inv_sum by auto
+
+end
